@prefix : <http://www.example.org/water#> .
@prefix rdfs: <http://www.w3.org/2000/01/rdf-schema#> .
:Water a rdfs:Class ;
    rdfs:label "Water" ;
    rdfs:comment "A liquid substance that covers most of the Earth's surface" .
:hasTemperature a rdfs:Property ;
    rdfs:domain :Water ;
    rdfs:range rdfs:Literal ;
    rdfs:label "has temperature" ;
    rdfs:comment "The property that describes the temperature of the water" .
:hasComposition a rdfs:Property ;
    rdfs:domain :Water ;
    rdfs:range :ChemicalCompound ;
    rdfs:label "has composition" ;
    rdfs:comment "The property that describes the chemical composition of the water" .
:ChemicalCompound a rdfs:Class ;
    rdfs:label "Chemical Compound" ;
    rdfs:comment "A chemical compound or substance consists of a fixed ratio of molecules or atoms" .
:H2O a :ChemicalCompound ;
    rdfs:label "H2O" ;
    rdfs:comment "H2O is the chemical formula for water, meaning each molecule of water consists of two hydrogen atoms bonded to a single oxygen atom" .
