@prefix rdf: <http://www.w3.org/1999/02/22-rdf-syntax-ns#> .
@prefix rdfs: <http://www.w3.org/2000/01/rdf-schema#> .
@prefix xsd: <http://www.w3.org/2001/XMLSchema#> .
@prefix ex: <http://example.org#> .
ex:Country a rdfs:Class ;
    rdfs:label "Country" ;
    rdfs:comment "A region identified as a distinct entity in political geography. A country may be an independent sovereign state or part of a larger state." .
ex:name a rdf:Property ;
    rdfs:label "name" ;
    rdfs:comment "The name of something." ;
    rdfs:domain ex:Country ;
    rdfs:range xsd:string .
ex:population a rdf:Property ;
    rdfs:label "population" ;
    rdfs:comment "The number of people who live in a country." ;
    rdfs:domain ex:Country ;
    rdfs:range xsd:integer .
ex:capital a rdf:Property ;
    rdfs:label "capital" ;
    rdfs:comment "The city that is the seat of government of a country." ;
    rdfs:domain ex:Country ;
    rdfs:range ex:City .
ex:City a rdfs:Class ;
    rdfs:label "City" ;
    rdfs:comment "A large human settlement. It can be either the capital or not." .
ex:area a rdf:Property ;
    rdfs:label "area" ;
    rdfs:comment "The quantifiable area a country covers, usually represented in square kilometers." ;
    rdfs:domain ex:Country ;
    rdfs:range xsd:float .
