@prefix rdf: <http://www.w3.org/1999/02/22-rdf-syntax-ns#> .
@prefix rdfs: <http://www.w3.org/2000/01/rdf-schema#> .
@prefix xsd: <http://www.w3.org/2001/XMLSchema#> .
@prefix home: <http://example.org/home#> .
home:Building a rdfs:Class ;
    rdfs:comment "A structure with walls and a roof." ;
    rdfs:label "Building" .
home:Apartment a rdfs:Class ;
    rdfs:label "Apartment" ;
    rdfs:comment "A suite of rooms forming one residence, typically in a building containing a number of these." ;
    rdfs:subClassOf home:Building .
    home:House a rdfs:Class ;
    rdfs:comment "A building for human habitation, especially one that is lived in by a family or small group of people." ;
    rdfs:label "House" ;
    rdfs:subClassOf home:Building .
    home:Room a rdfs:Class ;
    rdfs:comment "A part or division of a building enclosed by walls, floor, and ceiling." ;
    rdfs:label "Room" .
home:Kitchen a rdfs:Class ;
    rdfs:comment "A room or area where food is prepared and cooked." ;
    rdfs:label "Kitchen" ;
    rdfs:subClassOf home:Room .
home:Bathroom a rdfs:Class ;
    rdfs:comment "A room containing a bathtub or a shower and usually also a washbasin and a toilet." ;
    rdfs:label "Bathroom" ;
    rdfs:subClassOf home:Room .
home:hasRoom a rdf:Property ;
    rdfs:domain home:Building ;
    rdfs:range home:Room ;
    rdfs:label "has room" ;
    rdfs:comment "The property that relates a building with its rooms." .
