@prefix rdf: <http://www.w3.org/1999/02/22-rdf-syntax-ns#> .
@prefix rdfs: <http://www.w3.org/2000/01/rdf-schema#> .
@prefix owl: <http://www.w3.org/2002/07/owl#> .
@prefix xsd: <http://www.w3.org/2001/XMLSchema#> .
@prefix day: <http://example.org/day#> .
day:Day rdf:type owl:Class ;
    rdfs:comment "Class represents a generic day concept" ;
    rdfs:subClassOf rdfs:Resource .
day:hasTime rdf:type owl:ObjectProperty ;
    rdfs:comment "Property represents time segments in a day (morning, afternoon, evening, night)" ;
    rdfs:domain day:Day ;
    rdfs:range day:Time .
day:Time rdf:type owl:Class ;
    rdfs:comment "Class represents time periods in a day." ;
    rdfs:subClassOf rdfs:Resource .
day:Morning rdf:type owl:NamedIndividual, day:Time .
day:Afternoon rdf:type owl:NamedIndividual, day:Time .
day:Evening rdf:type owl:NamedIndividual, day:Time .
day:Night rdf:type owl:NamedIndividual, day:Time .
day:hasActivity rdf:type owl:ObjectProperty ;
    rdfs:comment "Property represents the activity done during a specific time of a day" ;
    rdfs:domain day:Time ;
    rdfs:range day:Activity .
day:Activity rdf:type owl:Class ;
    rdfs:comment "Class represents a type of activity that can be performed in a day." ;
    rdfs:subClassOf rdfs:Resource .
day:Work rdf:type owl:NamedIndividual, day:Activity .
day:Sleep rdf:type owl:NamedIndividual, day:Activity .
day:Eat rdf:type owl:NamedIndividual, day:Activity .
day:Play rdf:type owl:NamedIndividual, day:Activity .
day:hasDate rdf:type owl:DatatypeProperty ;
    rdfs:comment "Property represents the specific date for a day" ;
    rdfs:domain day:Day ;
    rdfs:range xsd:date .
