@prefix rdf: <http://www.w3.org/1999/02/22-rdf-syntax-ns#> .
@prefix rdfs: <http://www.w3.org/2000/01/rdf-schema#> .
@prefix xsd: <http://www.w3.org/2001/XMLSchema#> .
@prefix owl: <http://www.w3.org/2002/07/owl#> .
@prefix areaOnt: <http://example.org/ontology/area#> .
areaOnt:Area  rdf:type owl:Class ;
  rdfs:subClassOf areaOnt:PhysicalQuantity ;
  rdfs:label "Area" ;
  rdfs:comment "Area is a quantity that describes the extent of a two-dimensional surface or shape in the plane."@en ;
.areaOnt:hasArea  rdf:type owl:ObjectProperty ;
  rdfs:label "has area" ;
  rdfs:domain areaOnt:PhysicalObject ;
  rdfs:range areaOnt:Area ;
.areaOnt:PhysicalObject   rdf:type owl:Class ;
  rdfs:subClassOf owl:Thing ;
   rdfs:label "Physical Object" ;
  rdfs:comment "A physical object is a collection of matter within a defined contiguous boundary in three-dimensional space."@en ;
.areaOnt:PhysicalQuantity   rdf:type owl:Class ;
  rdfs:subClassOf owl:Thing ;
   rdfs:label "Physical Quantity" ;
  rdfs:comment "A physical quantity is a physical property of a phenomenon, body, or substance, that can be quantified by measurement."@en ;
.areaOnt:hasValue   rdf:type owl:DatatypeProperty ;
  rdfs:label "has value" ;
  rdfs:domain areaOnt:Area ;
  rdfs:range xsd:decimal ;
.areaOnt:hasUnit   rdf:type owl:ObjectProperty ;
  rdfs:label "has unit" ;
  rdfs:domain areaOnt:Area ;
  rdfs:range areaOnt:UnitOfMeasurement ;
.areaOnt:UnitOfMeasurement   rdf:type owl:Class ;
  rdfs:subClassOf owl:Thing ;
   rdfs:label "Unit of Measurement" ;
  rdfs:comment "Unit of measurement is a definite magnitude of a quantity, defined and adopted by convention or by law, that is used as a standard for measurement of the same kind of quantity."@en ;
.