@prefix rdfs: <http://www.w3.org/2000/01/rdf-schema#> .
@prefix owl: <http://www.w3.org/2002/07/owl#> .
@prefix xsd: <http://www.w3.org/2001/XMLSchema#> .
@prefix law: <http://example.org/law#> .
law:Law    rdfs:comment "An abstract concept which refers to the system of rules that a society or government develops in order to deal with crime, business agreements, social relationships, etc." ;
    a rdfs:Class .
law:CriminalLaw    rdfs:subClassOf law:Law ;
    rdfs:comment "A law that defines crimes against the public order." .
law:CivilLaw    rdfs:subClassOf law:Law ;
    rdfs:comment "A law that governs relationships between individuals and defines their legal rights." .
law:Lawyer    a rdfs:Class ;
    rdfs:comment "A person who practices or studies law." .
law:represents    a owl:ObjectProperty ;
    rdfs:domain law:Lawyer ;
    rdfs:range law:Law ;
    rdfs:comment "Represents an association between a lawyer and a particular segment of law." .
law:name    a owl:DatatypeProperty ;
    rdfs:domain law:Lawyer ;
    rdfs:range xsd:string ;
    rdfs:comment "Represents the name of a lawyer." .
law:hasExperienceIn    a owl:ObjectProperty ;
    rdfs:domain law:Lawyer ;
    rdfs:range law:Law ;
    rdfs:comment "Indicates a lawyer's experience in a particular area of law." .
law:Case    a rdfs:Class ;
    rdfs:comment "A legal dispute between two or more parties that is resolved by a court." .
law:happensInJurisdiction    a owl:ObjectProperty ;
    rdfs:domain law:Case ;
    rdfs:range law:Law ;
    rdfs:comment "Indicates the jurisdiction where a case happens." .
