@prefix rdf: <http://www.w3.org/1999/02/22-rdf-syntax-ns#> .
@prefix rdfs: <http://www.w3.org/2000/01/rdf-schema#> .
@prefix owl: <http://www.w3.org/2002/07/owl#> .
@prefix ex: <http://example.com/> .
ex:Head a rdfs:Class ;
  rdfs:comment "A part of the body at the top of the trunk, containing the brain, eyes, ears, nose, and mouth."@en ;
  rdfs:label "Head"@en .
ex:hasPart a rdf:Property ;
  rdfs:domain ex:Head ;
  rdfs:range rdfs:Class ;
  rdfs:comment "The parts that make up the head."@en ;
  rdfs:label "has part"@en .
ex:Ear a rdfs:Class ;
  rdfs:comment "One of the two organs of hearing, on either side of the head."@en ;
  rdfs:label "Ear"@en ;
  rdfs:subClassOf ex:Head .
ex:Eyes a rdfs:Class ;
  rdfs:comment "The pair of organs of sight, in humans and most animals, set in the head and enabled by light."@en ;
  rdfs:label "Eyes"@en ;
  rdfs:subClassOf ex:Head .
ex:Brain a rdfs:Class ;
  rdfs:comment "The organ inside the head that controls thought, memory, feelings, and activity."@en ;
  rdfs:label "Brain"@en ;
  rdfs:subClassOf ex:Head .
ex:Nose a rdfs:Class ;
  rdfs:comment "The part projecting above the mouth on the face of a person or animal, containing the nostrils and used for breathing and smelling."@en ;
  rdfs:label "Nose"@en ;
  rdfs:subClassOf ex:Head .
ex:Mouth a rdfs:Class ;
  rdfs:comment "The opening in the face used for speaking, eating, etc."@en ;
  rdfs:label "Mouth"@en ;
  rdfs:subClassOf ex:Head .
