@prefix : <http://www.example.org/#> .
@prefix rdf: <http://www.w3.org/1999/02/22-rdf-syntax-ns#> .
@prefix rdfs: <http://www.w3.org/2000/01/rdf-schema#> .
@prefix owl: <http://www.w3.org/2002/07/owl#> .
@prefix xsd: <http://www.w3.org/2001/XMLSchema#> .
:Member rdf:type owl:Class ;
      rdfs:label "Member" ;
      rdfs:comment "Representation of a member in a group or organization" .
:hasMember rdf:type owl:ObjectProperty ;
           rdfs:domain :Group ;
           rdfs:range :Member ;
           rdfs:label "has member" ;
           rdfs:comment "Relation between a group and an individual who is a member of that group" .
:memberOf rdf:type owl:ObjectProperty ;
           rdfs:domain :Member ;
           rdfs:range :Group ;
           rdfs:label "member of" ;
           rdfs:comment "Relation between an individual who is a member of a group and that group" .
:joinedDate rdf:type owl:DatatypeProperty ;
            rdfs:domain :Member ;
            rdfs:range xsd:date ;
            rdfs:label "date of joining" ;
            rdfs:comment "The date when the member joined the group" .
:name rdf:type owl:DatatypeProperty ;
      rdfs:domain :Member ;
      rdfs:range xsd:string ;
      rdfs:label "name" ;
      rdfs:comment "The name of the member" .
:Group rdf:type owl:Class ;
       rdfs:label "Group" ;
       rdfs:comment "Representation of a collection of individuals such as a team, club, association, or organization" .
