@prefix rdf: <http://www.w3.org/1999/02/22-rdf-syntax-ns#> .
@prefix rdfs: <http://www.w3.org/2000/01/rdf-schema#> .
@prefix xsd: <http://www.w3.org/2001/XMLSchema#> .
@prefix owl: <http://www.w3.org/2002/07/owl#> .
@prefix my: <http://example.org/WorldOntology#> .
my:World rdf:type owl:Class ;
    rdfs:label "World"@en ;
    rdfs:comment "This class represents the whole world including land masses, bodies of water, and life."my:Nations rdf:type owl:Class ;
    rdfs:subClassOf my:World ;
    rdfs:label "Nations"@en ;
    rdfs:comment "The class representing various nations in the world." .
my:Landmass rdf:type owl:Class ;
    rdfs:subClassOf my:World ;
    rdfs:label "Landmass"@en ;
    rdfs:comment "The class representing different landmasses present in the world." .
my:Ocean rdf:type owl:Class ;
    rdfs:subClassOf my:World ;
    rdfs:label "Ocean"@en ;
    rdfs:comment "This class represents the major oceans of the world." .
my:Life rdf:type owl:Class ;
    rdfs:subClassOf my:World ;
    rdfs:label "Life"@en ;
    rdfs:comment "This class represents all forms of life present in the world." .
my:population rdf:type owl:DatatypeProperty ;
    rdfs:domain my:Nations ;
    rdfs:range xsd:integer ;
    rdfs:label "population"@en ;
    rdfs:comment "This property indicates the population of specific nation." .
