@prefix rdf: <http://www.w3.org/1999/02/22-rdf-syntax-ns#> .
@prefix rdfs: <http://www.w3.org/2000/01/rdf-schema#> .
@prefix owl: <http://www.w3.org/2002/07/owl#> .
@prefix xsd: <http://www.w3.org/2001/XMLSchema#> .
@prefix level: <http://example.org/level#> .
level:     rdf:type owl:Ontology ;
    rdfs:comment "An ontology for levels"@en .
level:Level    rdf:type owl:Class ;
    rdfs:comment "Represents the concept of a level, it could be from a game, building or any concept that has different stratifications or tiers"@en ;
    rdfs:subClassOf owl:Thing .
level:hasLevelNumber    rdf:type owl:DatatypeProperty ;
    rdfs:comment "The property that represents the numeric representation of the level"@en ;
    rdfs:domain level:Level ;
    rdfs:range xsd:decimal .
level:hasLevelName    rdf:type owl:DatatypeProperty ;
    rdfs:comment "The property that represents the name of the level"@en ;
    rdfs:domain level:Level ;
    rdfs:range xsd:string .
level:hasLevelDifficulty    rdf:type owl:ObjectProperty ;
    rdfs:comment "The property that represents the difficulty of the level"@en ;
    rdf:domain level:Level ;
    rdf:range level:Difficulty .
level:hasNextLevel     rdf:type owl:ObjectProperty ;
    rdfs:comment "The property that represents the consecutive level after a current level"@en ;
    rdfs:domain level:Level ;
    rdfs:range level:Level .
level:Difficulty    rdf:type owl:Class ;
    rdfs:comment "Represents the concept of difficulty, generally categorized as 'easy,' 'medium' or 'hard'"@en ;
    rdfs:subClassOf owl:Thing .
level:Easy    rdf:type level:Difficulty .
level:Medium    rdf:type level:Difficulty .
level:Hard    rdf:type level:Difficulty .
