@prefix owl: <http://www.w3.org/2002/07/owl#> .
@prefix rdf: <http://www.w3.org/1999/02/22-rdf-syntax-ns#> .
@prefix rdfs: <http://www.w3.org/2000/01/rdf-schema#> .
@prefix xsd: <http://www.w3.org/2001/XMLSchema#> .
@prefix lv: <http://example.org/level#> .
# Classeslv:Level a rdfs:Class ;
    rdfs:subClassOf rdfs:Resource ;
    rdfs:label "Level" ;
    rdfs:comment "Represents a certain stage or position in a scale or series of increments." .
lv:LowLevel a rdfs:Class ;
    rdfs:subClassOf lv:Level ;
    rdfs:label "Low Level" ;
    rdfs:comment "Represents a stage or position that is considered below average in a series of levels." .
lv:MediumLevel a rdfs:Class ;
    rdfs:subClassOf lv:Level ;
    rdfs:label "Medium Level" ;
    rdfs:comment "Represents a stage or position that is considered average or normal in a series of levels." .
lv:HighLevel a rdfs:Class ;
    rdfs:subClassOf lv:Level ;
    rdfs:label "High Level" ;
    rdfs:comment "Represents a stage or position that is considered above average in a series of levels." .
# Propertieslv:hasLevel a rdf:Property ;
    rdfs:domain rdfs:Resource ;
    rdfs:range lv:Level ;
    rdfs:label "has level" ;
    rdfs:comment "Indicates the level associated with a certain object." .
