@prefix rdf: <http://www.w3.org/1999/02/22-rdf-syntax-ns#> .
@prefix rdfs: <http://www.w3.org/2000/01/rdf-schema#> .
@prefix owl: <http://www.w3.org/2002/07/owl#> .
@prefix xsd: <http://www.w3.org/2001/XMLSchema#> .
@base <http://example.org/office#> .
<http://example.org/office>    rdf:type owl:Ontology ;
    rdfs:comment "An ontology of the office domain"@en .
:Employee    rdf:type owl:Class ;
    rdfs:comment "A class of individuals who work in the office"@en ;
    rdfs:label "Employee"@en .
:Department    rdf:type owl:Class ;
    rdfs:comment "A class representing the different departments in the office"@en ;
    rdfs:label "Department"@en .
:officeEquipment    rdf:type owl:Class ;
    rdfs:comment "A class representing different office equipments"@en ;
    rdfs:label "Office Equipment"@en .
:worksIn    rdf:type owl:ObjectProperty ;
    rdfs:domain :Employee ;
    rdfs:range :Department ;
    rdfs:comment "A relation between an employee and the department they work in"@en ;
    rdfs:label "works in"@en .
:belongsTo    rdf:type owl:ObjectProperty ;
    rdfs:domain :officeEquipment ;
    rdfs:range :Department ;
    rdfs:comment "A relation between office equipment and the department it belongs to"@en ;
    rdfs:label "belongs to"@en .
:hasEmployee    rdf:type owl:ObjectProperty ;
    rdfs:domain :Department ;
    rdfs:range :Employee ;
    owl:inverseOf :worksIn ;
    rdfs:comment "A relation between a department and the employees who work in it"@en ;
    rdfs:label "has employee"@en .
:usesEquipment    rdf:type owl:ObjectProperty ;
    rdfs:domain :Employee ;
    rdfs:range :officeEquipment ;
    rdfs:comment "A relation between an employee and the equipment they use"@en ;
    rdfs:label "uses equipment"@en .
