@prefix rdfs: <http://www.w3.org/2000/01/rdf-schema#> .
@prefix ex: <http://example.org/#> .
ex:Money a rdfs:Class ;
     rdfs:label "Money" ;
    rdfs:comment "Entity that acts as a medium of exchange, a measure of value, a unit of account, and a store of value." ;
    rdfs:subClassOf ex:FinancialEntity .
ex:Currency a rdfs:Class ;
    rdfs:label "Currency" ;
    rdfs:comment "A system of money in general use in a particular country." ;
    rdfs:subClassOf ex:Money .
ex:DigitalCurrency a rdfs:Class ;
    rdfs:label "Digital currency" ;
    rdfs:comment "A type of currency available in digital form, represents money." ;
    rdfs:subClassOf ex:Money .
ex:hasValue a rdfs:Property ;
    rdfs:label "has value" ;
    rdfs:comment "Denotes the numerical value associated with a unit of money." ;
    rdfs:domain ex:Money ;
    rdfs:range rdfs:Literal .
