@prefix : <http://example.org/#> .
@prefix rdf: <http://www.w3.org/1999/02/22-rdf-syntax-ns#> .
@prefix rdfs: <http://www.w3.org/2000/01/rdf-schema#> .
@prefix xsd: <http://www.w3.org/2001/XMLSchema#> .
:Hand a rdfs:Class ;
rdfs:label "Hand"@en ;
rdfs:subClassOf :BodyPart ;
rdfs:comment "The hand is a human body part that is commonly used for grasping and manipulating objects."@en .
     :hasFingers a rdf:Property ;
    rdfs:label "has fingers"@en ;
    rdfs:domain :Hand ;
    rdfs:range :Finger .
:Finger a rdfs:Class ;
rdfs:label "Finger"@en ;
rdfs:subClassOf :BodyPart ;
rdfs:comment "A finger is a limb of the human body and a type of digit, a organ of manipulation and sensation found in the hands of humans."@en .
:BodyPart a rdfs:Class ;
rdfs:label "Body Part"@en ;
rdfs:comment "A body part is a part of an organism such as an animal or plant."@en .
