@prefix : <http://example.org/> .
@prefix rdf: <http://www.w3.org/1999/02/22-rdf-syntax-ns#> .
@prefix rdfs: <http://www.w3.org/2000/01/rdf-schema#> .
@prefix xsd: <http://www.w3.org/2001/XMLSchema#> .
:Chair rdf:type rdfs:Class ;
  rdfs:comment "A piece of furniture designed to accommodate one sitting or reclining person, providing support for the back and often the arms, and commonly standing on four legs."@en ;
  rdfs:subClassOf :Furniture .
:Furniture rdf:type rdfs:Class ;
  rdfs:label "Furniture"@en ;
  rdfs:comment "Items in a home, office, etc., such as tables, chairs, beds, or desks, used to make a space suitable for living or working."@en .
:hasMaterial rdf:type rdf:Property ;
  rdfs:domain :Furniture ;
  rdfs:range :Material ;
  rdfs:comment "The material from which a piece of furniture, like a chair, is made."@en .
:Material rdf:type rdfs:Class ;
  rdfs:comment "A substance that things can be made from."@en .
:Wood rdf:type :Material ;
  rdfs:comment "The hard fibrous material that forms the main substance of the trunk or branches of a tree or shrub."@en .
:Plastic rdf:type :Material ;
  rdfs:comment "Material consisting of any of a wide range of synthetic or semi-synthetic organic compounds that are malleable and so can be molded into solid objects."@en .
