@prefix rdf: <http://www.w3.org/1999/02/22-rdf-syntax-ns#> .
@prefix rdfs: <http://www.w3.org/2000/01/rdf-schema#> .
@prefix xsd: <http://www.w3.org/2001/XMLSchema#> .
@prefix game: <http://www.gameontology.org#> .
game:Game  rdf:type rdfs:Class ;
  rdfs:label "Game"@en ;
  rdfs:comment "A digital or non-digital activity that has rules and objectives"@en .
game:boardGame  rdf:type game:Game ;
  rdfs:label "Board Game"@en ;
  rdfs:comment "A game that involves counters or pieces moved or placed on a pre-marked surface or 'board', according to a set of rules"@en .
game:digitalGame  rdf:type game:Game ;
  rdfs:label "Digital Game"@en ;
  rdfs:comment "A game that is facilitated by electronic technology and can be played on devices like video game consoles, computers, smartphones etc."@en .
game:rolePlayingGame  rdf:type game:Game ;
  rdfs:label "Role Playing Game"@en ;
  rdfs:comment "A game in which players assume the roles of characters in a fictional setting"@en .
game:releaseYear  rdf:type rdf:Property ;
  rdfs:label "Release Year"@en ;
  rdfs:comment "The year when the game was released"@en ;
  rdfs:domain game:Game ;
  rdfs:range xsd:year .
game:rating  rdf:type rdf:Property ;
  rdfs:label "Rating"@en ;
  rdfs:comment "User rating of the game"@en ;
  rdfs:domain game:Game ;
  rdfs:range xsd:float .
