@prefix rdf: <http://www.w3.org/1999/02/22-rdf-syntax-ns#> .
@prefix rdfs: <http://www.w3.org/2000/01/rdf-schema#> .
@prefix time: <http://www.w3.org/2006/time#> .
time:Instant a rdfs:Class ;
    rdfs:label "Instant" ;
    rdfs:comment "An instant is a point on the time-line" .
time:Interval a rdfs:Class ;
    rdfs:label "Interval" ;
    rdfs:comment "A time interval is a duration on the time-line that is bounded by two instants" .
time:DateTimeDescription a rdfs:Class ;
    rdfs:label "DateTimeDescription" ;
    rdfs:comment "A description of date and time structured according to Gregorian calendar" .
time:inXSDDateTime a rdf:Property ;
    rdfs:range time:DateTimeDescription ;
    rdfs:domain time:Instant ;
    rdfs:label "in XSD datetime" ;
    rdfs:comment "Indicates the DateTimeDescription of the instant according to the xsd:dateTime format" .
time:hasBeginning a rdf:Property ;
    rdfs:range time:Instant ;
    rdfs:domain time:Interval ;
    rdfs:label "has beginning" ;
    rdfs:comment "Relation between a time interval and an instant at which it begins" .
time:hasEnd a rdf:Property ;
    rdfs:range time:Instant ;
    rdfs:domain time:Interval ;
    rdfs:label "has end" ;
    rdfs:comment "Relation between a time interval and an instant at which it ends" .
time:inXSDDuration a rdf:Property ;
    rdfs:range rdfs:Literal ;
    rdfs:domain time:Interval ;
    rdfs:label "in XSD duration" ;
    rdfs:comment "Indicates the duration of the interval in xsd:duration format" .
