@prefix rdf: <http://www.w3.org/1999/02/22-rdf-syntax-ns#> .
@prefix rdfs: <http://www.w3.org/2000/01/rdf-schema#> .
@prefix : <http://www.example.org/diabetes#> .
:Diabetes a rdfs:Class ;
    rdfs:label "Diabetes"@en ;
    rdfs:comment "A chronic disease that occurs either when the pancreas does not produce enough insulin or when the body cannot effectively use the insulin it produces."@en .
:Type1 a rdfs:Class ;
    rdfs:subClassOf :Diabetes ;
    rdfs:label "Type 1 Diabetes"@en ;
    rdfs:comment "A form of diabetes that results from the autoimmune destruction of the insulin-producing beta cells in the pancreas."@en .
:Type2 a rdfs:Class ;
    rdfs:subClassOf :Diabetes ;
    rdfs:label "Type 2 Diabetes"@en ;
    rdfs:comment "A metabolic disorder that is primarily characterized by insulin resistance, relative insulin deficiency, and hyperglycemia."@en .
:Gestational a rdfs:Class ;
    rdfs:subClassOf :Diabetes ;
    rdfs:label "Gestational Diabetes"@en ;
    rdfs:comment "A form of high blood sugar affecting pregnant women."@en .
   :Hyperglycemia a rdfs:Class ;
    rdfs:label "Hyperglycemia "@en ;
    rdfs:comment "A condition of abnormally high blood glucose level, which is a characteristic symptom of diabetes."@en .
:Insulin a rdfs:Class ;
    rdfs:label "Insulin"@en ;
    rdfs:comment "A hormone produced in pancreas to regulate the amount of glucose in the blood."@en .
   :Diabetes rdfs:seeAlso :Hyperglycemia, :Insulin .
:Type1 rdfs:disjointWith :Type2, :Gestational .
:Type2 rdfs:disjointWith :Gestational .
