@prefix rdf: <http://www.w3.org/1999/02/22-rdf-syntax-ns#> .
@prefix rdfs: <http://www.w3.org/2000/01/rdf-schema#> .
@prefix xsd: <http://www.w3.org/2001/XMLSchema#> .
@prefix work: <http://example.com/work#> .
work:Work rdfs:subClassOf rdf:Property ;
    rdfs:label "Work"@en .
work:employee rdfs:subClassOf work:Work ;
    rdfs:label "Employee"@en ;
    rdfs:comment "A person who is hired to provide services to a company regularly in exchange for compensation and does not provide these services as part of an independent business."@en .
work:employer rdfs:subClassOf work:Work ;
    rdfs:label "Employer"@en ;
    rdfs:comment "A legal entity that controls and directs a servant or worker under an express or implied contract of employment and pays them salary or wages in return."@en .
work:position rdfs:subClassOf work:Work ;
    rdfs:label "Position"@en ;
    rdfs:comment "Job title or role defined by its responsibilities or duties."@en .
work:salary rdf:type rdf:Property ;
    rdfs:label "Salary"@en ;
    rdfs:comment "Regular payment from employer to employee."@en ;
    rdfs:domain work:employee ;
    rdfs:range xsd:decimal .
work:company rdf:type rdf:Property ;
    rdfs:label "Company"@en ;
    rdfs:comment "An organized group of people with a particular purpose, such as a business or government department."@en ;
    rdfs:domain work:employer ;
    rdfs:range xsd:string .
work:hasPosition rdf:type rdf:Property ;
    rdfs:label "Has position"@en ;
    rdfs:comment "An employee holds a particular position in an organization."@en ;
    rdfs:domain work:employee ;
    rdfs:range work:position .
