@prefix rdfs: <http://www.w3.org/2000/01/rdf-schema#> .
@prefix rdf: <http://www.w3.org/1999/02/22-rdf-syntax-ns#> .
@prefix ex: <http://example.org/> .
ex:Result     rdf:type rdfs:Class ;
    rdfs:label "Result" ;
    rdfs:comment "This Class represents outcomes of any process" .
ex:hasResult     rdf:type rdf:Property ;
    rdfs:label "hasResult" ;
    rdfs:comment "The property that links any process to its outcome" ;
    rdfs:domain ex:Process ;
    rdfs:range ex:Result .
ex:isResultOf     rdf:type rdf:Property ;
    rdfs:label "isResultOf" ;
    rdfs:comment "The property that links any result to its corresponding process" ;
    rdfs:domain ex:Result ;
    rdfs:range ex:Process .
ex:Process     rdf:type rdfs:Class ;
    rdfs:label "Process" ;
    rdfs:comment "This Class represents any procedure that can yield a result" .
ex:hasProcess     rdf:type rdf:Property ;
    rdfs:label "hasProcess" ;
    rdfs:comment "The property that links any agent or actor to the process it performs" ;
    rdfs:domain ex:Agent ;
    rdfs:range ex:Process .
ex:Agent     rdf:type rdfs:Class ;
    rdfs:label "Agent" ;
    rdfs:comment "This Class represents any entity capable of carrying out a process to produce a result" .
