@prefix rdf: <http://www.w3.org/1999/02/22-rdf-syntax-ns#> .
@prefix rdfs: <http://www.w3.org/2000/01/rdf-schema#> .
@prefix xsd: <http://www.w3.org/2001/XMLSchema#> .
@prefix impact: <http://www.example.org/ontology/impact#> .
impact:Impact     rdf:type rdfs:Class ;
    rdfs:label "Impact"@en ;
    rdfs:comment "Represents the effect that a certain action, decision, or event has upon entities or environments."@en ;
.impact:hasMagnitude    rdf:type rdf:Property ;
    rdfs:label "has magnitude"@en ;
    rdfs:comment "The measure of the size, extent or importance of an impact."@en ;
    rdfs:domain impact:Impact ;
    rdfs:range xsd:float ;
.impact:hasTarget     rdf:type rdf:Property ;
    rdfs:label "has target"@en ;
    rdfs:comment "The entity or environment targeted by the action, decision, or event causing the impact."@en ;
    rdfs:domain impact:Impact ;
.impact:hasCause     rdf:type rdf:Property ;
    rdfs:label "has cause"@en ;
    rdfs:comment "The action, decision, or event causing the impact."@en ;
    rdfs:domain impact:Impact ;
.impact:isPositive    rdf:type rdf:Property ;
    rdfs:label "is positive"@en ;
    rdfs:comment "True if the impact is positive or beneficial;
 false if it is negative or harmful."@en ;
    rdfs:domain impact:Impact ;
    rdfs:range xsd:boolean ;
.impact:Event     rdf:type rdfs:Class ;
    rdfs:label "Event"@en ;
    rdfs:comment "Represents an action, decision, or happening that can cause impacts."@en ;
.impact:Entity     rdf:type rdfs:Class ;
    rdfs:label "Entity"@en ;
    rdfs:comment "Represents an entity that can be affected by impacts."@en ;
.