@prefix rdf: <http://www.w3.org/1999/02/22-rdf-syntax-ns#> .
@prefix owl: <http://www.w3.org/2002/07/owl#> .
@prefix rdfs: <http://www.w3.org/2000/01/rdf-schema#> .
@prefix xsd: <http://www.w3.org/2001/XMLSchema#> .
@prefix way: <http://www.example.org/way#> .
way:   rdf:type owl:Ontology ;
  rdfs:comment "Ontology of the concept Way"@en .
way:Way   rdf:type owl:Class ;
  rdfs:label "Way"@en ;
  rdfs:comment "Abstract representation of a way, path, route or means to achieve something or to reach a destination."@en .
way:Direction  rdf:type owl:Class ;
  rdfs:label "Direction"@en ;
  rdfs:comment "Representation of the orientation or course taken by a way."@en ;
  rdfs:subClassOf way:Way .
way:Journey   rdf:type owl:Class ;
  rdfs:label "Journey"@en ;
  rdfs:comment "Specific series of paths or routes taken as part of a way to a destination."@en ;
  rdfs:subClassOf way:Way .
  way:Guide   rdf:type owl:Class ;
  rdfs:label "Guide"@en ;
  rdfs:comment "Entity that helps anyone to determine the best way or the path that should be taken."@en .
way:guide   rdf:type owl:ObjectProperty ;
  rdfs:label "guide"@en ;
  rdfs:comment "Relation to represent the guide of a way."@en ;
  rdfs:domain way:Way ;
  rdfs:range way:Guide .
way:hasDirection   rdf:type owl:DatatypeProperty ;
  rdfs:label "hasDirection"@en ;
  rdfs:comment "Relation to represent the direction a specific way is heading to."@en ;
  rdfs:domain way:Way ;
  rdfs:range xsd:string .
  way:hasJourney   rdf:type owl:DatatypeProperty ;
  rdfs:label "hasJourney"@en ;
  rdfs:comment "Relation to depict the journey of a specific way."@en ;
  rdfs:domain way:Way ;
  rdfs:range xsd:string .
