@prefix : <http://www.example.org/thing#> .
@prefix rdfs: <http://www.w3.org/2000/01/rdf-schema#> .
@prefix owl: <http://www.w3.org/2002/07/owl#> .
@prefix xsd: <http://www.w3.org/2001/XMLSchema#> .
:Thing a rdfs:Class ;
    rdfs:label "Thing"@en ;
    rdfs:comment "A conceptual entity that can be real, virtual, abstract or physical."@en ;
.:hasName a owl:DatatypeProperty ;
    rdfs:domain :Thing ;
    rdfs:range xsd:string ;
    rdfs:comment "The name of the thing."@en ;
.:hasDescription a owl:DatatypeProperty ;
    rdfs:domain :Thing ;
    rdfs:range xsd:string ;
    rdfs:comment "A description of the thing."@en ;
.:PhysicalThing rdfs:subClassOf :Thing ;
    rdfs:label "Physical Thing"@en ;
    rdfs:comment "A thing that is physical and can be interacted with materially."@en ;
.:AbstractThing rdfs:subClassOf :Thing ;
    rdfs:label "Abstract Thing"@en ;
    rdfs:comment "A thing that is abstract and cannot be interacted with materially."@en ;
.:CreatedThing rdfs:subClassOf :Thing ;
    rdfs:label "Created Thing"@en ;
    rdfs:comment "A thing that was created or made by an agent."@en ;
.:NaturalThing rdfs:subClassOf :Thing ;
    rdfs:label "Natural Thing"@en ;
    rdfs:comment "A thing that was not made or created by an agent, but exists naturally."@en ;
.
