@prefix rdf: <http://www.w3.org/1999/02/22-rdf-syntax-ns#> .
@prefix rdfs: <http://www.w3.org/2000/01/rdf-schema#> .
@prefix owl: <http://www.w3.org/2002/07/owl#> .
@prefix : <http://example.com/thing#> .
# Thing Ontology :Thing rdf:type owl:Class ;
  rdfs:label "Thing" ;
  rdfs:comment "A universal entity in the universe i.e everything is a thing" ;
  owl:axiom [    a owl:Axiom ;
    owl:propertyChainAxiom ( :partOf :isMadeOf ) ;
    owl:annotatedTarget :Thing ;
    owl:annotatedSource :Thing ;
    owl:annotatedProperty owl:equivalentClass   ] ;
  rdfs:subClassOf owl:Thing .
:isMadeOf rdf:type owl:ObjectProperty ;
  rdfs:domain :Thing ;
  rdfs:range :Thing ;
  rdfs:label "is made of" ;
  rdfs:comment "Relates a thing to what it is made of, which is also a thing." .
:partOf rdf:type owl:ObjectProperty ;
  rdfs:domain :Thing ;
  rdfs:range :Thing ;
  rdfs:label "part of" ;
  rdfs:comment "Relates a thing to what it is part of, which is also a thing." .
