@prefix : <http://www.example.com/ontology/world#> .
@prefix rdf: <http://www.w3.org/1999/02/22-rdf-syntax-ns#> .
@prefix rdfs: <http://www.w3.org/2000/01/rdf-schema#> .
@prefix xsd: <http://www.w3.org/2001/XMLSchema#> .
: a rdfs:Ontology ;
  rdfs:label "World Ontology"@en ;
  rdfs:comment "An ontology describing concepts related to the world"@en .
:Country a rdfs:Class ;
  rdfs:label "Country"@en ;
  rdfs:comment "A nation with its own government, occupying a particular territory"@en .
:City a rdfs:Class ;
  rdfs:label "City"@en ;
  rdfs:comment "A large town or a populated area of a country"@en .
:CityWithin rdfs:SubPropertyOf rdf:Property ;
  rdfs:domain :City ;
  rdfs:range :Country ;
  rdfs:label "city within"@en ;
  rdfs:comment "A city that is within a certain country"@en .
:Population a rdf:Property ;
  rdfs:domain :Country ;
  rdfs:range xsd:integer ;
  rdfs:label "Population"@en ;
  rdfs:comment "The number of people living in a country"@en .
:Continent a rdfs:Class ;
  rdfs:label "Continent"@en ;
  rdfs:comment "A principal division of the Earth's surface"@en .
:CountryWithin rdfs:SubPropertyOf rdf:Property ;
  rdfs:domain :Country ;
  rdfs:range :Continent ;
  rdfs:label "country within"@en ;
  rdfs:comment "A country that is within a certain continent"@en .
:Language a rdfs:Class ;
  rdfs:label "Language"@en ;
  rdfs:comment "A system of communication used by a particular country or community"@en .
:OfficialLanguage a rdf:Property ;
  rdfs:domain :Country ;
  rdfs:range :Language ;
  rdfs:label "Official language"@en ;
  rdfs:comment "The language recognised as the 'official' language of a country"@en .
