@prefix rdfs: <http://www.w3.org/2000/01/rdf-schema#> .
@prefix owl: <http://www.w3.org/2002/07/owl#> .
@prefix rdf: <http://www.w3.org/1999/02/22-rdf-syntax-ns#> .
@prefix xsd: <http://www.w3.org/2001/XMLSchema#> .
@prefix : <http://example.org/life#> .
:Life rdfs:label "Life"@en .
:Life rdfs:comment "Represents the concept life as it exists in a diverse forms on earth."@en .
:Human rdfs:subClassOf :Life .
:Human rdfs:label "Human"@en .
:Human rdfs:comment "Represents the human specie of life on earth."@en .
:Animal rdfs:subClassOf :Life .
:Animal rdfs:label "Animal"@en .
:Animal rdfs:comment "Represents the concept of animal as a form of life on earth."@en .
:Plant rdfs:subClassOf :Life .
:Plant rdfs:label "Plant"@en .
:Plant rdfs:comment "Represents the concept of plant as a form of life on earth."@en .
:Microorganism rdfs:subClassOf :Life .
:Microorganism rdfs:label "Microorganism"@en .
:Microorganism rdfs:comment "Represents the concept of microorganisms as a form of life on earth."@en .
:bornIn rdf:type owl:ObjectProperty .
:bornIn rdfs:domain :Life .
:bornIn rdfs:range :Location .
:bornIn rdfs:label "born in"@en .
:diedIn rdf:type owl:ObjectProperty .
:diedIn rdfs:domain :Life .
:diedIn rdfs:range :Location .
:diedIn rdfs:label "died in"@en .
