@prefix rdf: <http://www.w3.org/1999/02/22-rdf-syntax-ns#> .
@prefix rdfs: <http://www.w3.org/2000/01/rdf-schema#> .
@prefix xsd: <http://www.w3.org/2001/XMLSchema#> .
@prefix owl: <http://www.w3.org/2002/07/owl#> .
@prefix way: <http://www.semanticweb.org/ontology/way#> .
way:Way  rdf:type owl:Class ;
  rdfs:comment "Secondary concept that represents different types of ways in which something can be done or exist" ;
  rdfs:subClassOf owl:Thing .
way:PhysicalWay  rdf:type owl:Class ;
  rdfs:comment "Way that involves physical actions or processes" ;
  rdfs:subClassOf way:Way .
way:MentalWay  rdf:type owl:Class ;
  rdfs:comment "Way that involves mental actions or processes" ;
  rdfs:subClassOf way:Way .
way:TechnologicalWay  rdf:type owl:Class ;
  rdfs:comment "Way that involves technological methods or processes" ;
  rdfs:subClassOf way:Way .
way:direction  rdf:type owl:ObjectProperty ;
  rdfs:domain way:Way ;
  rdfs:range way:Direction .
way:Way  rdf:type owl:Class ;
  rdfs:comment "Main concept that signify any course along which someone or something may move." .
way:Direction  rdf:type owl:Class ;
  rdfs:comment "Subconcept to describe a course or route along which something travels or moves." .
way:hasSpeed   rdf:type owl:DatatypeProperty ;
  rdfs:domain way:Way ;
  rdfs:range xsd:float ;
  rdfs:comment "The attribute indicating the speed at which an entity is moving along a way." .
