@prefix rdf: <http://www.w3.org/1999/02/22-rdf-syntax-ns#> .
@prefix owl: <http://www.w3.org/2002/07/owl#> .
@prefix xsd: <http://www.w3.org/2001/XMLSchema#> .
@prefix rdfs: <http://www.w3.org/2000/01/rdf-schema#> .
@prefix : <http://www.example.org/world_ontology#> .
: a owl:Ontology ;
:World a owl:Class ;
    rdfs:label "World"@en ;
    rdfs:comment "This class represents the concept of World, the planet Earth"@en .
    :Country a owl:Class ;
    rdfs:subClassOf :World ;
    rdfs:label "Country"@en ;
    rdfs:comment "This class represents the concept of Country, a nation within the World"@en .
    :City a owl:Class ;
    rdfs:subClassOf :Country ;
    rdfs:label "City"@en ;
    rdfs:comment "This class represents the concept of City, a city within a Country"@en .
:isPartOf a owl:ObjectProperty ;
    rdfs:domain :City ;
    rdfs:range :Country ;
    rdfs:label "is part of"@en ;
    rdfs:comment "This property links a City to the Country it is part of"@en .
