@prefix ex: <http://example.org/> .
@prefix rdf: <http://www.w3.org/1999/02/22-rdf-syntax-ns#> .
@prefix rdfs: <http://www.w3.org/2000/01/rdf-schema#> .
@prefix owl: <http://www.w3.org/2002/07/owl#> .
ex:World rdf:type rdfs:Class ;
          rdfs:comment "The planet Earth and everything on it." ;
          rdfs:subClassOf ex:Universe .
ex:Continent rdf:type rdfs:Class ;
             rdfs:comment "Any of the world's main continuous expanses of land." ;
             rdfs:subClassOf ex:World .
ex:Ocean rdf:type rdfs:Class ;
         rdfs:comment "The vast body of salt water that covers almost three fourths of the earth's surface." ;
         rdfs:subClassOf ex:World .
ex:Country rdf:type rdfs:Class ;
           rdfs:comment "A nation with its own government, occupying a particular territory." ;
           rdfs:subClassOf ex:Continent .
ex:City rdf:type rdfs:Class ;
        rdfs:comment "A large town." ;
        rdfs:subClassOf ex:Country .
ex:Mountain rdf:type rdfs:Class ;
            rdfs:comment "A large natural elevation of the earth's surface rising abruptly from the surrounding level;
 a large hill." ;
            rdfs:subClassOf ex:Continent .
ex:River rdf:type rdfs:Class ;
         rdfs:comment "A large natural stream of water flowing in a channel to the sea, a lake, or another river." ;
         rdfs:subClassOf ex:Continent .
ex:Lake rdf:type rdfs:Class ;
        rdfs:comment "A large body of water surrounded by land." ;
        rdfs:subClassOf ex:Continent .
