@prefix rdf: <http://www.w3.org/1999/02/22-rdf-syntax-ns#> .
@prefix rdfs: <http://www.w3.org/2000/01/rdf-schema#> .
@prefix xsd: <http://www.w3.org/2001/XMLSchema#> .
@prefix water: <http://www.example.com/water#> .
water:     rdf:type rdfs:Class ;
    rdfs:label "Water"@en;
    rdfs:comment "The liquid that forms the seas, lakes, rivers, and rain and is the basis of the fluids of living organisms."@en .
water:State    rdf:type rdfs:Class ;
    rdfs:label "State"@en ;
    rdfs:comment "The different physical states in which water can exist: solid (ice), liquid (water), and gas (steam or vapor)."@en .
    water:Source      rdf:type rdfs:Class ;
    rdfs:label "Source"@en ;
    rdfs:comment "The origin points or places where water is sourced from, such as rivers, lakes, oceans, wells, etc."@en .
water:hasState    rdf:type rdf:Property ;
    rdfs:domain water: ;
    rdfs:range water:State ;
    rdfs:label "has state"@en ;
    rdfs:comment "The property that relates water to its physical state."@en .
water:hasSource    rdf:type rdf:Property ;
    rdfs:domain water: ;
    rdfs:range water:Source ;
    rdfs:label "has source"@en ;
    rdfs:comment "The property that relates water to its source."@en .
## Instances of water in different stateswater:IcelandGlacierWater    rdf:type water: ;
    water:hasState water:Solid ;
    water:hasSource "Glacier"^^xsd:string ;
    rdfs:label "Iceland Glacier water"@en .
water:AmazonRiverWater    rdf:type water: ;
    water:hasState water:Liquid ;
    water:hasSource "River"^^xsd:string ;
    rdfs:label "Amazon River water"@en .
water:BoilingWater    rdf:type water: ;
    water:hasState water:Gas ;
    water:hasSource "Kettle"^^xsd:string ;
    rdfs:label "Boiling water"@en .
