@prefix rdf: <http://www.w3.org/1999/02/22-rdf-syntax-ns#> .
@prefix owl: <http://www.w3.org/2002/07/owl#> .
@prefix rdfs: <http://www.w3.org/2000/01/rdf-schema#> .
@prefix war: <http://example.org/ontology/war#> .
war:War rdf:type owl:Class ;
    rdfs:label "War" ;
    rdfs:subClassOf rdfs:Thing ;
    rdfs:comment "Represents the occurrence of an armed conflict between different nations or states or different groups within a nation or state." .
    war:involvedParty rdf:type owl:ObjectProperty ;
        rdfs:label "involved party" ;
        rdfs:comment "Designates the nations, states, or groups involved in a war." ;
        rdfs:domain war:War ;
        rdfs:range rdfs:Thing .
     war:startTime rdf:type owl:DatatypeProperty ;
        rdfs:label "start time" ;
        rdfs:comment "Designates the date when a war started." ;
        rdfs:domain war:War ;
        rdfs:range rdf:langString .
    war:endTime rdf:type owl:DatatypeProperty ;
        rdfs:label "end time" ;
        rdfs:comment "Designates the date when a war ended." ;
        rdfs:domain war:War ;
        rdfs:range rdf:langString .
    war:hasCasualties rdf:type owl:DatatypeProperty ;
        rdfs:label "has casualties" ;
        rdfs:comment "Designates the number of individuals killed, injured or missing in a war." ;
        rdfs:domain war:War ;
        rdfs:range rdf:langString .
    war:causedBy rdf:type owl:ObjectProperty ;
        rdfs:label "caused by" ;
        rdfs:comment "Designates the primary causes that lead to the occurrence of a war." ;
        rdfs:domain war:War ;
        rdfs:range rdfs:Thing .
