# Defining Base URI and Prefixes@base <http://example.org/history/> .
@prefix rdf: <http://www.w3.org/1999/02/22-rdf-syntax-ns#> .
@prefix rdfs: <http://www.w3.org/2000/01/rdf-schema#> .
@prefix xsd: <http://www.w3.org/2001/XMLSchema#> .
# Class
:History a rdfs:Class;
         rdfs:comment "All events that have occurred in the past".
:HistoricalEvent a rdfs:Class;
                rdfs:comment "An occurrence within human history".
:HistoricalPeriod a rdfs:Class;
                 rdfs:comment "A length of time singled out because of specific events, trends, innovations, or high culture".
:HistoricalFigure a rdfs:Class;
                 rdfs:comment "Any person who has significantly influenced the course of history".
                 # Properties
:hasEvent a rdf:Property;
             rdfs:domain :History;
             rdfs:range :HistoricalEvent;
             rdfs:comment "Relates a period of history to the events that occurred during that time".
:hasPeriod a rdf:Property;
              rdfs:domain :History;
              rdfs:range :HistoricalPeriod;
              rdfs:comment "Relates a period of history to the larger history".
:hasFigure a rdf:Property;
           rdfs:domain :History;
           rdfs:range :HistoricalFigure;
           rdfs:comment "Relates a figure to the period or event within which they were influential".
:eventOccurredDuring a rdf:Property;
           rdfs:domain :HistoricalEvent;
           rdfs:range :HistoricalPeriod;
           rdfs:comment "Relates an event to the period during which it occurred".
:figureLivedDuring a rdf:Property;
           rdfs:domain :HistoricalFigure;
           rdfs:range :HistoricalPeriod;
           rdfs:comment "Relates a figure to the period during which they lived and/or were influential".
