@prefix xsd: <http://www.w3.org/2001/XMLSchema#> .
@prefix ex: <http://example.org/> .
ex:Eye     a ex:BodyOrgan ;
    ex:hasPart ex:Lens ;
    ex:hasPart ex:Cornea ;
    ex:hasPart ex:Iris ;
    ex:hasPart ex:Retina ;
    ex:linkedTo ex:OpticNerve ;
    ex:characteristic "Vision"^^xsd:string .
 ex:Lens    a ex:EyeComponent ;
    ex:function "Focusing light"^^xsd:string .
ex:Cornea    a ex:EyeComponent ;
    ex:function "Protecting the eye"^^xsd:string .
ex:Iris    a ex:EyeComponent ;
    ex:function "Controlling the diameter and size of the pupil"^^xsd:string .
ex:Retina    a ex:EyeComponent ;
    ex:function "Receiving light that the lens has focused, turning it into neural signals"^^xsd:string .
ex:OpticNerve    a ex:BodyOrgan ;
    ex:function "Transmitting visual information from the retina to the brain"^^xsd:string .
ex:BodyOrgan    a rdfs:Class ;
    rdfs:comment "Body organs are parts of an organism which perform vital body functions."^^xsd:string .
ex:EyeComponent     a rdfs:Class ;
    rdfs:comment "Eye components not only help to protect the eye but are also vital in the process of seeing."^^xsd:string .
ex:hasPart    a rdf:Property ;
    rdfs:domain ex:BodyOrgan ;
    rdfs:range ex:EyeComponent ;
    rdfs:comment "This property links body organs to their components."^^xsd:string .
ex:linkedTo    a rdf:Property ;
    rdfs:domain ex:BodyOrgan ;
    rdfs:range ex:BodyOrgan ;
    rdfs:comment "This property describes which body organs are linked to each other."^^xsd:string .
ex:function    a rdf:Property ;
    rdfs:domain [ rdf:type owl:Class ;
 owl:unionOf ( ex:EyeComponent ex:BodyOrgan ) ] ;
    rdfs:range xsd:string ;
    rdfs:comment "This property gives the function of body organs or eye components."^^xsd:string .
ex:characteristic    a rdf:Property ;
    rdfs:domain ex:BodyOrgan ;
    rdfs:range xsd:string ;
    rdfs:comment "This property gives the characteristic of a body organ."^^xsd:string .
