 This is expressed in Turtle RDF which is a standard language for Semantic Web technologies like ontology:
@prefix xsd: <http://www.w3.org/2001/XMLSchema#> .
@prefix time: <http://www.example.org/ontology/time#> .
time:Time a rdfs:Class ;
          rdfs:comment "This is a fundamental class representing time" .
time:Hour a rdfs:Class ;
           rdfs:subClassOf time:Time ;
           rdfs:comment "This represents the smaller unit of time, the hour" .
time:Minute a rdfs:Class ;
             rdfs:subClassOf time:Hour ;
             rdfs:comment "This represents the smaller unit of time, the minute. 60 minutes make an hour." .
time:lengthInHours a rdf:Property ;
                   rdfs:domain time:Time ;
                   rdfs:range xsd:float ;
                   rdfs:comment "This property denotes the length of a certain time span in terms of hours" .
time:lengthInMinutes a rdf:Property ;
                   rdfs:domain time:Time ;
                   rdfs:range xsd:float ;
                   rdfs:comment "This property denotes the length of a certain time span in terms of minutes" .
