@prefix rdf: <http://www.w3.org/1999/02/22-rdf-syntax-ns#> .
@prefix rdfs: <http://www.w3.org/2000/01/rdf-schema#> .
@prefix xsd: <http://www.w3.org/2001/XMLSchema#> .
@prefix air: <http://example.org/ontology/air#> .
air:     rdf:type rdfs:Class ;
    rdfs:label "Air"@en ;
    rdfs:comment "The invisible gaseous substance surrounding the earth, a mixture mainly of oxygen and nitrogen."@en .
air:Composition     rdf:type rdfs:Class ;
    rdfs:label "Composition"@en ;
    rdfs:comment "The details about the different components of air."@en .
air:Nitrogen     rdf:type rdfs:Class ;
    rdfs:label "Nitrogen"@en ;
    rdfs:comment "A colorless, odorless gaseous element that constitutes about four-fifths of the volume of the atmosphere."@en .
    air:Oxygen     rdf:type rdfs:Class ;
    rdfs:label "Oxygen"@en ;
    rdfs:comment "A colorless, odorless reactive gaseous element that is life-supporting, constituting about one fifth of the air."@en .
air:hasPart     rdf:type rdf:Property ;
    rdfs:label "has part"@en ;
    rdfs:comment "Relates air to its components."@en ;
    rdfs:domain air: ;
    rdfs:range air:Composition .
air:percentage     rdf:type rdf:Property ;
    rdfs:label "percentage"@en ;
    rdfs:comment "The part of air a component constitutes expressed as a percentage"@en ;
    rdfs:domain air:Composition ;
    rdfs:range xsd:decimal .
    air:AirQuality    rdf:type rdfs:Class;
    rdfs:label "Air Quality"@en;
    rdfs:comment "The degree to which air is free from pollution"@en. air:Pollutant     rdf:type rdfs:Class;
    rdfs:label "Pollutant"@en;
    rdfs:comment "A substance that has been introduced to the atmosphere that has harmful or poisonous effects"@en.    air:contains    rdf:type rdf:Property;
    rdfs:label "contains"@en;
    rdfs:comment "Relates air to any pollutants it contains"@en;
    rdfs:domain air:AirQuality;
    rdfs:range air:Pollutant.