@prefix rdf: <http://www.w3.org/1999/02/22-rdf-syntax-ns#> .
@prefix rdfs: <http://www.w3.org/2000/01/rdf-schema#> .
@prefix owl: <http://www.w3.org/2002/07/owl#> .
@prefix xsd: <http://www.w3.org/2001/XMLSchema#> .
@prefix air: <http://example.org/air#> .
# Class
 air:Air     rdf:type owl:Class ;
    rdfs:comment "Air is the general name for the mixture of gases that makes up the Earth's atmosphere."@en ;
    rdfs:subClassOf owl:Thing .
air:NaturalAir     rdf:type owl:Class ;
    rdfs:comment "Natural air is air in its natural state, with no artificial additives or changes."@en ;
    rdfs:subClassOf air:Air .
air:PollutedAir     rdf:type owl:Class ;
    rdfs:comment "Polluted air contains contaminants or substances harmful or poisonous to organisms."@en ;
    rdfs:subClassOf air:Air .
# Properties
air:contains     rdf:type owl:ObjectProperty ;
    rdfs:comment "The property that defines what an air consists of."@en ;
    rdfs:domain air:Air ;
    rdfs:range air:Component .
air:quality     rdf:type owl:DatatypeProperty ;
    rdfs:comment "The property that describes the quality of air."@en ;
    rdfs:domain air:Air ;
    rdfs:range xsd:string .
# Individuals
air:Oxygen    rdf:type air:Component ;
    rdfs:comment "One of the gases that makes up the air we breathe in"@en .
air:Nitrogen    rdf:type air:Component ;
    rdfs:comment "The most abundant gas in the Earth's atmosphere"@en .
