@prefix rdf: <http://www.w3.org/1999/02/22-rdf-syntax-ns#> .
@prefix rdfs: <http://www.w3.org/2000/01/rdf-schema#> .
@prefix owl: <http://www.w3.org/2002/07/owl#> .
@prefix xsd: <http://www.w3.org/2001/XMLSchema#> .
@prefix : <http://example.org/force#> .
:Force a rdfs:Class ;
    rdfs:comment "Represents the physical quantity that can cause a change in the motion of an object" ;
    rdfs:label "Force" .
:Magnitude a rdfs:Datatype ;
    rdfs:subClassOf xsd:decimal ;
    rdfs:label "Magnitude" ;
    rdfs:comment "The magnitude (or strength or size) of the force. It's a measure of how strong the force is."@en .
:direction a rdfs:Property ;
    rdfs:domain :Force ;
    rdfs:range xsd:string ;
    rdfs:comment "The direction of the force which indicates exactly where the force is pointed"@en ;
    rdfs:label "Direction"@en .
:hasMagnitude a rdfs:Property ;
    rdfs:domain :Force ;
    rdfs:range :Magnitude ;
    rdfs:label "Has Magnitude" ;
    rdfs:comment "Relates a force to its magnitude." .
