```turtle@prefix : <http://example.org/ontology/cost#> .@prefix rdf: <http://www.w3.org/1999/02/22-rdf-syntax-ns#> .@prefix rdfs: <http://www.w3.org/2000/01/rdf-schema#> .@prefix xsd: <http://www.w3.org/2001/XMLSchema#> .:Cost a rdfs:Class ;    rdfs:label "Cost" ;    rdfs:comment "A monetary or other value required to acquire, produce, accomplish, or maintain something." .:FixedCost a rdfs:Class ;    rdfs:subClassOf :Cost ;    rdfs:label "Fixed Cost" ;    rdfs:comment "A cost that does not change with an increase or decrease in the amount of goods or services produced." .:VariableCost a rdfs:Class ;    rdfs:subClassOf :Cost ;    rdfs:label "Variable Cost" ;    rdfs:comment "A cost that varies with the level of output." .:SemiVariableCost a rdfs:Class ;    rdfs:subClassOf :Cost ;    rdfs:label "Semi-Variable Cost" ;    rdfs:comment "A cost composed of a mixture of fixed and variable components." .:DirectCost a rdfs:Class ;    rdfs:subClassOf :Cost ;    rdfs:label "Direct Cost" ;    rdfs:comment "A cost that can be directly attributed to a specific product or activity." .:IndirectCost a rdfs:Class ;    rdfs:subClassOf :Cost ;    rdfs:label "Indirect Cost" ;    rdfs:comment "A cost that cannot be directly attributed to a specific product or activity." .:hasAmount a rdf:Property ;    rdfs:domain :Cost ;    rdfs:range xsd:decimal ;    rdfs:label "has amount" ;    rdfs:comment "The monetary value of the cost." .:hasCurrency a rdf:Property ;    rdfs:domain :Cost ;    rdfs:range xsd:string ;    rdfs:label "has currency" ;    rdfs:comment "The currency in which the cost is measured." .:hasCostType a rdf:Property ;    rdfs:domain :Cost ;    rdfs:range :Cost ;    rdfs:label "has cost type" ;    rdfs:comment "The classification of the cost as fixed, variable, etc." .```