"@prefix rdf: <http://www.w3.org/1999/02/22-rdf-syntax-ns#> .
@prefix rdfs: <http://www.w3.org/2000/01/rdf-schema#> .
@prefix xsd: <http://www.w3.org/2001/XMLSchema#> .
@prefix pms: <http://www.example.org/precision/machining/service#> .
pms:MachiningService    rdf:type rdfs:Class ;
    rdfs:comment ""A class representing precision machining services""^^xsd:string ;
    rdfs:label ""MachiningService""^^xsd:string .
pms:Machine    rdf:type rdfs:Class ;
    rdfs:comment ""A class representing the machine used in precision machining""^^xsd:string ;
    rdfs:label ""Machine""^^xsd:string .
pms:Material    rdf:type rdfs:Class ;
    rdfs:comment ""A class representing the material subject to precision machining""^^xsd:string ;
    rdfs:label ""Material""^^xsd:string .
pms:usesMachine    rdf:type rdf:Property ;
    rdfs:comment ""A property linking a machining service to a machine""^^xsd:string ;
    rdfs:domain pms:MachiningService ;
    rdfs:range pms:Machine ;
    rdfs:label ""usesMachine""^^xsd:string .
pms:processMaterial    rdf:type rdf:Property ;
    rdfs:comment ""A property linking a machining service to a material""^^xsd:string ;
    rdfs:domain pms:MachiningService ;
    rdfs:range pms:Material ;
    rdfs:label ""processMaterial""^^xsd:string .
pms:precisionLevel    rdf:type rdf:Property ;
    rdfs:comment ""A property representing the precision level of the machining service""^^xsd:string ;
    rdfs:domain pms:MachiningService ;
    rdfs:range xsd:int ;
    rdfs:label ""precisionLevel""^^xsd:string .
"