@prefix rdf: <http://www.w3.org/1999/02/22-rdf-syntax-ns#> .
@prefix rdfs: <http://www.w3.org/2000/01/rdf-schema#> .
@prefix foaf: <http://xmlns.com/foaf/0.1/> .
@prefix hf: <http://example.org/homelessFamily#> .
hf:Family a rdfs:Class ;
    rdfs:comment ""A group of people united by certain conviction or common affiliation. In this case, family without home.""@en .
    hf:Member a rdfs:Class ;
    rdfs:comment ""An individual that belongs to a family.""@en ;
    rdfs:subClassOf foaf:Person .
    hf:hasMember a rdf:Property ;
    rdfs:comment ""Relates a family to a person who is a member of that family.""@en ;
    rdfs:domain hf:Family ;
    rdfs:range hf:Member .
hf:isMemberOf a rdf:Property ;
    rdfs:comment ""Relates a person to a family to which they belong.""@en ;
    rdfs:domain hf:Member ;
    rdfs:range hf:Family .
hf:Homelessness a rdfs:Class ;
    rdfs:comment ""The state or condition of having no home or permanent place of residence.""@en .
hf:isHomeless a rdf:Property ;
    rdfs:comment ""Indicates whether a family or an individual is homeless or not.""@en ;
    rdfs:domain [ rdf:type owl:Class ;
 owl:unionOf ( hf:Family hf:Member ) ] ;
    rdfs:range hf:Homelessness .
hf:Support a rdfs:Class ;
    rdfs:comment ""Assistance provided to homeless families or individuals.""@en .
hf:receivesSupport a rdf:Property ;
    rdfs:comment ""Indicates the support received by a homeless family or individual.""@en ;
    rdfs:domain hf:Homelessness ;
    rdfs:range hf:Support .
hf:providesSupport a rdf:Property ;
    rdfs:comment ""Indicates the entity providing support to homeless families or individuals.""@en ;
    rdfs:domain hf:Support ;
    rdfs:range [ rdf:type owl:Class ;
 owl:unionOf ( hf:Family hf:Member ) ] .
