@prefix rdf: <http://www.w3.org/1999/02/22-rdf-syntax-ns#> .
@prefix rdfs: <http://www.w3.org/2000/01/rdf-schema#> .
@prefix xsd: <http://www.w3.org/2001/XMLSchema#> .
@prefix back: <http://example.org/back#> .
back:Back a rdfs:Class ;
    rdfs:label "Back" ;
    rdfs:comment "A class that represents the concept of 'Back' or 'Rear' in a spatial or conceptual sense.".
back:hasLocation a rdf:Property ;
    rdfs:range xsd:string ;
    rdfs:domain back:Back ;
    rdfs:comment "A property that indicates the location of 'Back' in a given context." .
back:isBackOf a rdf:Property ;
    rdfs:range back:Back ;
    rdfs:comment "A property that indicates what 'Back' is behind or is the rear of." .
back:isOppositeOf a rdf:Property ;
    rdfs:range xsd:string ;
    rdfs:domain back:Back ;
    rdfs:comment "A property that indicates what is opposite of 'Back'." .
