@prefix : <http://example.org/> .
:Back a owl:Class ;
    rdfs:subClassOf :Body_Part ;
    rdfs:comment "The part of the body from the neck to the end of the spine" ;
    rdfs:label "Back" .
:Upper_Back a owl:Class ;
    rdfs:subClassOf :Back ;
    rdfs:comment "The upper half of the back consisting of shoulders to the bottom of the rib cage" ;
    rdfs:label "Upper Back" .
:Lower_Back a owl:Class ;
    rdfs:subClassOf :Back ;
    rdfs:comment "The lower half of the back extending from the bottom of the rib cage to the end of the spine" ;
    rdfs:label "Lower Back" .
:Spine a owl:Class ;
    rdfs:subClassOf :Back ;
    rdfs:comment "The series of vertebrae extending from the skull to the small of the back" ;
    rdfs:label "Spine" .
:Lumbar_Spine a owl:Class ;
    rdfs:subClassOf :Spine ;
    rdfs:comment "The lower section of the spine, generally consisting of five vertebrae" ;
    rdfs:label "Lumbar Spine" .
:Thoracic_Spine a owl:Class ;
    rdfs:subClassOf :Spine ;
    rdfs:comment "The middle and largest section of the spine, generally consisting of twelve vertebrae" ;
    rdfs:label "Thoracic Spine" .
:Cervical_Spine a owl:Class ;
    rdfs:subClassOf :Spine ;
    rdfs:comment "The top section of the spine, usually consisting of seven vertebrae" ;
    rdfs:label "Cervical Spine" .
