@prefix rdf: <http://www.w3.org/1999/02/22-rdf-syntax-ns#> .
@prefix rdfs: <http://www.w3.org/2000/01/rdf-schema#> .
@prefix xsd: <http://www.w3.org/2001/XMLSchema#> .
@prefix ex: <http://example.com/> .
ex:Minute rdf:type rdfs:Class ;
    rdfs:label "Minute"@en ;
    rdfs:comment "A unit of time equal to 60 seconds"@en ;
    rdfs:subClassOf ex:Time .
ex:secondInMinute rdf:type rdf:Property ;
    rdfs:label "second in minute"@en ;
    rdfs:comment "The number of seconds in a minute"@en ;
    rdfs:domain ex:Minute ;
    rdfs:range xsd:Integer .
    ex:secondInMinute rdfs:subPropertyOf ex:secondInTime .
ex:minuteInHour rdf:type rdf:Property ;
    rdfs:label "minute in hour"@en ;
    rdfs:comment "The number of minutes in an hour"@en ;
    rdfs:domain ex:Hour ;
    rdfs:range ex:Minute .
    ex:minuteInHour rdfs:subPropertyOf ex:minuteInTime .
ex:Time rdf:type rdfs:Class ;
    rdfs:label "Time"@en ;
    rdfs:comment "A dimension in which events can be ordered from the past through the present into the future"@en .
ex:secondInTime rdf:type rdf:Property ;
    rdfs:label "second in time"@en ;
    rdfs:comment "The standard unit of time in the International System of Units (SI)"@en ;
    rdfs:domain ex:Time ;
    rdfs:range xsd:Integer .
ex:minuteInTime rdf:type rdf:Property ;
    rdfs:label "minute in time"@en ;
    rdfs:comment "A unit of time used universally to understand chronological order"@en ;
    rdfs:domain ex:Time ;
    rdfs:range ex:Minute .
