@prefix rdf: <http://www.w3.org/1999/02/22-rdf-syntax-ns#> .
@prefix rdfs: <http://www.w3.org/2000/01/rdf-schema#> .
@prefix : <http://example.com/system#> .
:System a rdfs:Class ;
    rdfs:label "System" ;
    rdfs:comment "The class of all systems" .
:SubSystem a rdfs:Class ;
    rdfs:subClassOf :System ;
    rdfs:comment "The class of all subsystems, which are systems in their own right but also part of a larger system" .
:OperatingSystem a rdfs:Class ;
    rdfs:subClassOf :System ;
    rdfs:label "Operating System" ;
    rdfs:comment "A software that, after being initially loaded into the computer by a boot program, manages all of the other application programs in a computer" .
:SystemComponent a rdfs:Class ;
    rdfs:label "System Component" ;
    rdfs:comment "An individual part of a system" .
:partOf a rdf:Property ;
    rdfs:domain :SystemComponent ;
    rdfs:range :System ;
    rdfs:label "is part of" ;
    rdfs:comment "A relation between a system component and the system it is a part of" .
 :hasComponent a rdf:Property ;
    rdfs:domain :System ;
    rdfs:range :SystemComponent ;
    rdfs:label "has component" ;
    rdfs:comment "A relation between a system and a component it has" .
