@prefix rdf: <http://www.w3.org/1999/02/22-rdf-syntax-ns#> .
@prefix rdfs: <http://www.w3.org/2000/01/rdf-schema#> .
@prefix owl: <http://www.w3.org/2002/07/owl#> .
@prefix xsd: <http://www.w3.org/2001/XMLSchema#> .
@prefix time: <http://www.example.org/time#> .
time:Time    rdf:type rdfs:Class ;
    rdfs:label "Time" ;
    rdfs:comment "Representation of time which can be broken up into days, hours, minutes or seconds" .
time:hasUnit    rdf:type rdf:Property ;
    rdfs:label "hasUnit" ;
    rdfs:range time:TimeUnit ;
    rdfs:domain time:Time ;
    rdfs:comment "Property to represent the unit of time for a specific interval" .
time:TimeUnit    rdf:type rdfs:Class ;
    rdfs:label "Time Unit" ;
    rdfs:subClassOf time:Time ;
    rdfs:comment "Units used to represent time e.g. days, hours, minutes and seconds" .
time:hour    rdf:type time:TimeUnit ;
    rdfs:label "hour" .
time:minute    rdf:type time:TimeUnit ;
    rdfs:label "minute" .
time:second    rdf:type time:TimeUnit ;
    rdfs:label "second" .
time:day    rdf:type time:TimeUnit ;
    rdfs:label "day" .
time:quantity    rdf:type rdf:Property ;
    rdfs:label "quantity" ;
    rdfs:domain time:Time ;
    rdfs:range xsd:int ;
    rdfs:comment "Property to denote the number quantity for a time entity" .
