@prefix rdf: <http://www.w3.org/1999/02/22-rdf-syntax-ns#> .
@prefix rdfs: <http://www.w3.org/2000/01/rdf-schema#> .
@prefix owl: <http://www.w3.org/2002/07/owl#> .
@prefix xsd: <http://www.w3.org/2001/XMLSchema#> .
@prefix time: <http://www.w3.org/2006/time#> .
time:TimeInterval rdf:type owl:Class ;
    rdfs:label "Time Interval"@en ;
    rdfs:comment "An interval of time."@en .
time:Instant rdf:type owl:Class ;
    rdfs:label "Instant"@en ;
    rdfs:comment "A specific point in time."@en ;
    rdfs:subClassOf time:TimeInterval .
time:TemporalEntity rdf:type owl:Class ;
    rdfs:label "Temporal Entity"@en ;
    rdfs:comment "Any entity that has temporal extent or location."@en .
time:hasTime rdf:type owl:ObjectProperty ;
    rdfs:label "has time"@en ;
    rdfs:comment "Relates an entity to the TimeIntervals at which it is present."@en ;
    rdfs:domain time:TemporalEntity ;
    rdfs:range time:TimeInterval .
time:inXSDDate rdf:type owl:DatatypeProperty ;
    rdfs:label "in XSD Date"@en ;
    rdfs:comment "Relates an instant or interval of time with its representation as an xsd:Date."@en ;
    rdfs:domain [ rdf:type owl:Class ;
 owl:unionOf (time:Instant time:TimeInterval) ] ;
    rdfs:range xsd:Date .
time:before rdf:type owl:ObjectProperty ;
    rdfs:label "before"@en ;
    rdfs:comment "Indicates that one time interval is completely before another."@en ;
    rdfs:domain time:TimeInterval ;
    rdfs:range time:TimeInterval .
time:after rdf:type owl:ObjectProperty ;
    rdfs:label "after"@en ;
    rdfs:comment "Indicates that one time interval is completely after another."@en ;
    rdfs:domain time:TimeInterval ;
    rdfs:range time:TimeInterval .
