@prefix : <http://www.example.com/water#> .
@prefix rdf: <http://www.w3.org/1999/02/22-rdf-syntax-ns#> .
@prefix rdfs: <http://www.w3.org/2000/01/rdf-schema#> .
@prefix owl: <http://www.w3.org/2002/07/owl#> .
@prefix xsd: <http://www.w3.org/2001/XMLSchema#> .
: a owl:Ontology ;
  rdfs:comment "This is a simple water ontology."@en .
:Lake a owl:Class ;
  owl:disjointWith :River ;
  rdfs:comment "A type of body of water which is larger than a pond and is usually formed as a result of geological activity."@en .
  :River a owl:Class ;
  owl:disjointWith :Lake ;
  rdfs:comment "A type of body of water that flows downhill usually ending in a sea or an ocean."@en .
:WaterProperty   a owl:Class ;
  rdfs:comment "The characteristics or attributes associated to water."@en .
:hasWaterProperty   a owl:ObjectProperty ;
  rdfs:domain :Lake, :River ;
  rdfs:range :WaterProperty ;
  rdfs:comment "The property is used to associate bodies of water to their features."@en .
  :Temperature   a owl:Class ;
  rdfs:subClassOf :WaterProperty ;
  rdfs:comment "The degree or intensity of heat present in water."@en .
  :PH   a owl:Class ;
  rdfs:subClassOf :WaterProperty ;
  rdfs:comment "The pH of water is a measure of how acidic or alkaline it is."@en .
:WaterCycle  a owl:Class ;
  rdfs:comment "The process by which water circulates on earth."@en .
:Evaporation   a owl:Class ;
  rdfs:subClassOf :WaterCycle ;
  rdfs:comment "The process where water is converted from liquid to vapor."@en .
  :Condensation   a owl:Class ;
  rdfs:subClassOf :WaterCycle ;
  rdfs:comment "The process where water vapor cools down and turns into liquid water."@en .
:Precipitation   a owl:Class ;
  rdfs:subClassOf :WaterCycle ;
  rdfs:comment "The process where water falls from the sky in the form of rain, snow, hail or sleet."@en .
