@prefix xsd: <http://www.w3.org/2001/XMLSchema#> .
@prefix rdf: <http://www.w3.org/1999/02/22-rdf-syntax-ns#> .
@prefix rdfs: <http://www.w3.org/2000/01/rdf-schema#> .
@prefix ex: <http://example.org/> .
ex:Level a rdfs:Class ;
  rdfs:label "Level"@en ;
  rdfs:comment "A class representing various categories of levels."@en .
ex:hasDifficulty a rdf:Property ;
  rdfs:domain ex:Level ;
  rdfs:range xsd:string ;
  rdfs:label "hasDifficulty"@en ;
  rdfs:comment "The property represents the difficulty level of a certain level."@en .
ex:hasNumber a rdf:Property ;
  rdfs:domain ex:Level ;
  rdfs:range xsd:integer ;
  rdfs:label "hasNumber"@en ;
  rdfs:comment "The property that represents the sequencing number of a level."@en .
ex:hasReward a rdf:Property ;
  rdfs:domain ex:Level ;
  rdfs:range xsd:string ;
  rdfs:label "hasReward"@en ;
  rdfs:comment "The property that represents the reward obtained after completing a level."@en .
ex:inGame a rdf:Property ;
  rdfs:domain ex:Level ;
  rdfs:range ex:Game ;
  rdfs:label "inGame"@en ;
  rdfs:comment "The property that links a level to the game in which it is found."@en .
ex:Game a rdfs:Class ;
  rdfs:label "Game"@en ;
  rdfs:comment "This class represents games in which levels can be found."@en .
