@prefix rdf: <http://www.w3.org/1999/02/22-rdf-syntax-ns#> .
@prefix rdfs: <http://www.w3.org/2000/01/rdf-schema#> .
@prefix owl: <http://www.w3.org/2002/07/owl#> .
@prefix xsd: <http://www.w3.org/2001/XMLSchema#> .
@prefix word: <http://www.example.org/word#> .
word:Word rdf:type owl:Class ;
          rdfs:comment "Represents a word in general sense" .
word:hasSpelling rdf:type owl:DatatypeProperty ;
                 rdfs:domain word:Word ;
                 rdfs:range xsd:string ;
                 rdfs:comment "The spelling of the word" .
word:hasLemma rdf:type owl:DatatypeProperty ;
              rdfs:domain word:Word ;
              rdfs:range xsd:string ;
              rdfs:comment "The lemma or dictionary form of the word" .
word:hasPartOfSpeech rdf:type owl:ObjectProperty ;
                     rdfs:domain word:Word ;
                     rdfs:range word:PartOfSpeech ;
                     rdfs:comment "The part of speech of the word" .
word:Noun rdf:type owl:NamedIndividual, word:PartOfSpeech ;
          rdfs:label "Noun" ;
          rdfs:comment "A part of speech that is usually used to refer to a person, place, or thing" .
word:Verb rdf:type owl:NamedIndividual, word:PartOfSpeech ;
          rdfs:label "Verb" ;
          rdfs:comment "A part of speech that describes an action, occurrence, or state of being".
word:Adjective rdf:type owl:NamedIndividual, word:PartOfSpeech ;
               rdfs:label "Adjective" ;
               rdfs:comment "A part of speech that modifies a noun or pronoun" .
word:Adverb rdf:type owl:NamedIndividual, word:PartOfSpeech ;
            rdfs:label "Adverb" ;
            rdfs:comment "A part of speech that modifies a verb, an adjective, another adverb, a phrase, or a clause" .
