@prefix rdf: <http://www.w3.org/1999/02/22-rdf-syntax-ns#> .
@prefix rdfs: <http://www.w3.org/2000/01/rdf-schema#> .
@prefix owl: <http://www.w3.org/2002/07/owl#> .
@prefix air: <http://www.example.org/ontology/air#> .
air: a owl:Ontology;
  rdfs:comment "An ontology dedicated to Air".
air:Air a owl:Class;
  rdfs:label "Air";
  rdfs:comment "The mixture of gases that surrounds the earth and forms its atmosphere".
air:Atmosphere a owl:Class;
  rdfs:subClassOf air:Air;
  rdfs:label "Atmosphere";
  rdfs:comment "The gaseous envelope surrounding the earth;
 the air".
air:Troposphere a owl:Class;
  rdfs:subClassOf air:Atmosphere;
  rdfs:label "Troposphere";
  rdfs:comment "The lowest region of the atmosphere, extending from the earth's surface to a height of about 6â€“10 km".
air:AirPollution a owl:Class;
  rdfs:subClassOf air:Air;
  rdfs:label "Air pollution";
  rdfs:comment "The presence in or introduction into the air of a substance which has harmful or poisonous effects".
air:GreenhouseGas a owl:Class;
  rdfs:subClassOf air:Air;
  rdfs:label "Greenhouse Gas";
  rdfs:comment "A gas that contributes to the greenhouse effect by absorbing infrared radiation".
air:airComponent a owl:ObjectProperty;
  rdfs:domain air:Air;
  rdfs:range air:Air;
  rdfs:label "is a component of";
  rdfs:comment "Relates an air portion to the air it is a component of".
air:hasAirQuality a owl:DataProperty;
  rdfs:domain air:Air;
  rdfs:range rdf:literal;
  rdfs:label "has air quality";
  rdfs:comment "Property that denotes the quality of air, usually expressed in terms of pollutant concentrations".
