@prefix xsd: <http://www.w3.org/2001/XMLSchema#> .
@prefix rdf: <http://www.w3.org/1999/02/22-rdf-syntax-ns#> .
@prefix rdfs: <http://www.w3.org/2000/01/rdf-schema#> .
@prefix : <http://handontologyexample.org/> .
:Hand a rdfs:Class ;
    rdfs:comment "A human's appendage that can manipulate objects" .
    :Thumb a :Hand ;
    rdfs:comment "The first digit of the hand, located most laterally" .
    :IndexFinger a :Hand ;
    rdfs:comment "The second digit of the hand, located central to the thumb and middle finger" .
    :MiddleFinger a :Hand ;
    rdfs:comment "The third digit of the hand, located central to the index and ring finger" .
   :RingFinger a :Hand ;
    rdfs:comment "The fourth digit of the hand, located central to the middle finger and little finger" .
    :LittleFinger a :Hand ;
    rdfs:comment "The fifth and smallest digit of the hand, located most medially" .
:hasFingers a rdf:Property ;
    rdfs:domain :Hand ;
    rdfs:range xsd:string ;
    rdfs:comment "The number of fingers on a hand" .
:hasThumb a rdf:Property ;
    rdfs:domain :Hand ;
    rdfs:range xsd:boolean ;
    rdfs:comment "Indicates if a hand has a thumb or not".
    :canGrasp a rdf:Property ;
    rdfs:domain :Hand ;
    rdfs:range xsd:boolean ;
    rdfs:comment "Indicates if a hand can grasp objects or not" .
