@prefix rdf: <http://www.w3.org/1999/02/22-rdf-syntax-ns#> .
@prefix rdfs: <http://www.w3.org/2000/01/rdf-schema#> .
@prefix xsd: <http://www.w3.org/2001/XMLSchema#> .
@prefix ex: <http://example.org/place#> .
##Class definitionsex:Country a rdfs:Class ;
    rdfs:label "Country"@en ;
    rdfs:comment "A nation with its own government, occupying a particular territory."@en .
ex:State a rdfs:Class ;
    rdfs:label "State"@en ;
    rdfs:comment "An organized political community under one government within a country."@en ;
    rdfs:subClassOf ex:Country .
ex:City a rdfs:Class ;
    rdfs:label "City"@en ;
    rdfs:comment "A large town created by human with residential, business and other purposes."@en ;
    rdfs:subClassOf ex:State .
##Property definitionsex:hasCapital a rdf:Property ;
    rdfs:label "capital"@en ;
    rdfs:comment "The city that is the seat of government of a country or a state."@en ;
    rdfs:domain ex:Country ;
    rdfs:range ex:City .
ex:hasPopulation a rdf:Property ;
    rdfs:label "population"@en ;
    rdfs:comment "The number of people that live in a country, state or city."@en ;
    rdfs:domain ex:Country ;
    rdfs:range xsd:integer .
ex:hasArea a rdf:Property ;
    rdfs:label "area"@en ;
    rdfs:comment "The geographical area a country, state or city occupies."@en ;
    rdfs:domain ex:Country ;
    rdfs:range xsd:Decimal .
