@prefix rdf: <http://www.w3.org/1999/02/22-rdf-syntax-ns#> .
@prefix rdfs: <http://www.w3.org/2000/01/rdf-schema#> .
@prefix ex: <http://example.com/> .
ex:Word a rdfs:Class ;
  rdfs:label "Word" ;
  rdfs:comment "A unit of language that functions as a principal carrier of meaning." .
  ex:hasSpelling a rdf:Property ;
  rdfs:range xsd:string ;
  rdfs:domain ex:Word ;
  rdfs:label "has spelling" ;
  rdfs:comment "The specific arrangement of letters that forms a particular word." .
ex:hasDefinition a rdf:Property ;
  rdfs:range xsd:string ;
  rdfs:domain ex:Word ;
  rdfs:label "has definition" ;
  rdfs:comment "The meaning of the word." .
ex:hasPartOfSpeech a rdf:Property ;
  rdfs:range ex:PartOfSpeech ;
  rdfs:domain ex:Word ;
  rdfs:label "has part of speech" ;
  rdfs:comment "The role the word plays in a sentence, e.g., noun, verb, etc." .
  ex:PartOfSpeech a rdfs:Class ;
  rdfs:label "Part of Speech" ;
  rdfs:comment "The grammatical term that deals with the roles words play when used in the context of a sentence." .
