@prefix rdf: <http://www.w3.org/1999/02/22-rdf-syntax-ns#> .
@prefix rdfs: <http://www.w3.org/2000/01/rdf-schema#> .
@prefix owl: <http://www.w3.org/2002/07/owl#> .
@prefix xsd: <http://www.w3.org/2001/XMLSchema#> .
@prefix fo: <http://www.example.com/ForceOntology#> .
fo:Force a rdfs:Class ;
    rdfs:label "Force" ;
    rdfs:comment "The entity that causes a change in motion of an object" .
fo:Magnitude a rdfs:Class ;
    rdfs:subClassOf fo:Force ;
    rdfs:label "Magnitude" ;
    rdfs:comment "The size of the force which is usually measured in newtons (N)" .
fo:Direction a rdfs:Class ;
    rdfs:subClassOf fo:Force ;
    rdfs:label "Direction" ;
    rdfs:comment "The direction indicating where the force is applied" .
fo:AppliedForce a rdfs:Class ;
    rdfs:subClassOf fo:Force ;
    rdfs:label "Applied Force" ;
    rdfs:comment "The force which is applied to an object by another object" .
fo:FrictionForce a rdfs:Class ;
    rdfs:subClassOf fo:Force ;
    rdfs:label "Friction Force" ;
    rdfs:comment "The force resisting the relative motion of solid surfaces, fluid layers, and material elements" .
fo:GravitationalForce a rdfs:Class ;
    rdfs:subClassOf fo:Force ;
    rdfs:label "Gravitational Force" ;
    rdfs:comment "The force with which the earth, moon, or other massively large object attracts another object towards itself " .
fo:object1 a fo:Force ;
    fo:magnitude "20"^^xsd:int ;
    fo:direction "North" ;
    fo:appliedForce "Push" ;
    fo:frictionForce "5"^^xsd:int ;
    fo:gravitationalForce "9.8"^^xsd:float .
