@prefix rdf: <http://www.w3.org/1999/02/22-rdf-syntax-ns#> .
@prefix rdfs: <http://www.w3.org/2000/01/rdf-schema#> .
@prefix owl: <http://www.w3.org/2002/07/owl#> .
@prefix xsd: <http://www.w3.org/2001/XMLSchema#> .
@prefix law: <http://www.example.org/law/> .
law:Law  rdf:type rdfs:Class ;
  rdfs:comment "A system of rules and guidelines which are enforced through social institutions to govern behavior" ;
  rdfs:label "Law" .
law:CaseLaw  rdf:type rdfs:Class ;
  rdfs:subClassOf law:Law ;
  rdfs:comment "Law that is based on judicial decisions rather than statutes" ;
  rdfs:label "Case Law" .
law:StatutoryLaw  rdf:type rdfs:Class ;
  rdfs:subClassOf law:Law ;
  rdfs:comment "Written law set down by a body of legislature or by a singular legislator" ;
  rdfs:label "Statutory Law" .
law:CriminalLaw  rdf:type rdfs:Class ;
  rdfs:subClassOf law:Law ;
  rdfs:comment "Body of law which relates to crime" ;
  rdfs:label "Criminal Law" .
law:CivilLaw  rdf:type rdfs:Class ;
  rdfs:subClassOf law:Law ;
  rdfs:comment "Branch of law dealing with disputes between individuals and/or organizations" ;
  rdfs:label "Civil Law" .
law:Lawyer  rdf:type rdfs:Class ;
  rdfs:comment "A professional who practices or studies law" ;
  rdfs:label "Lawyer" .
law:practicesLaw  rdf:type rdf:Property ;
  rdfs:domain law:Lawyer ;
  rdfs:range law:Law ;
  rdfs:comment "Specifies that a person practices a particular type or branch of law" ;
  rdfs:label "practices law" .
law:passedBy  rdf:type rdf:Property ;
  rdfs:domain law:StatutoryLaw ;
  rdfs:range rdfs:Resource ;
  rdfs:comment "Specifies the entity which passed the law" ;
  rdfs:label "passed by" .
law:court  rdf:type rdfs:Class ;
  rdfs:comment "Institution presiding over the application of law";
  rdfs:label "Court" .
law:judges   rdf:type rdf:Property ;
  rdfs:domain law:court ;
  rdfs:range rdfs:Resource ;
  rdfs:comment "Specifies the judges in a court" ;
  rdfs:label "has judges".
