@prefix rdf: <http://www.w3.org/1999/02/22-rdf-syntax-ns#> .
@prefix rdfs: <http://www.w3.org/2000/01/rdf-schema#> .
@prefix govt: <http://example.org/govt#> .
govt:Government  rdf:type rdfs:Class ;
  rdfs:comment "The organization that is the governing authority of a political unit" ;
  rdfs:label "Government" .
govt:Department  rdf:type rdfs:Class ;
  rdfs:comment "A specialised division of a government" ;
  rdfs:label "Department" ;
  rdfs:subClassOf govt:Government .
govt:leaderOf  rdf:type rdf:Property ;
  rdfs:domain govt:Person ;
  rdfs:range govt:Government ;
  rdfs:comment "A person who is the leader or head of a government or department" ;
  rdfs:label "leaderOf" .
govt:Person  rdf:type rdfs:Class ;
  rdfs:comment "A human being" ;
  rdfs:label "Person" .
govt:legislation  rdf:type rdf:Property ;
  rdfs:domain govt:Government ;
  rdfs:range govt:Law ;
  rdfs:comment "The process of making or enacting laws" ;
  rdfs:label "legislation" .
govt:Law  rdf:type rdfs:Class ;
  rdfs:comment "A rule enacted or customary in a community and recognised as enjoining or prohibiting certain actions" ;
  rdfs:label "Law" .
