@prefix xsd: <http://www.w3.org/2001/XMLSchema#> .
@prefix right: <http://example.org/right#> .
@prefix dbpedia: <http://dbpedia.org/resource/> .
right:Right a owl:Class ;
    rdfs:comment "The concept of legal, ethical, moral, or natural rights" ;
    rdfs:subClassOf dbpedia:Social_concepts .
right:HumanRight a owl:Class ;
    rdfs:comment "Rights inherent to all human beings, regardless of race, sex, nationality, ethnicity, language, religion, or any other status" ;
    rdfs:subClassOf right:Right .
right:PropertyRight a owl:Class ;
    rdfs:comment "Theoretical legally enforceable powers to control use of property" ;
    rdfs:subClassOf right:Right .
right:AnimalRight a owl:Class ;
    rdfs:comment "Idea that non-human animals should be regarded as persons and members of the moral community" ;
    rdfs:subClassOf right:Right .
right:CivilRight a owl:Class ;
    rdfs:comment "Class of rights that protect individuals' freedom from infringement by governments, social organizations, and private individuals" ;
    rdfs:subClassOf right:Right .
right:RightDirection a owl:Class ;
    rdfs:comment "Direction that is the opposite of left" ;
    rdfs:subClassOf dbpedia:Direction .
right:RightTriangle a owl:Class ;
    rdfs:comment "Triangle in which one angle is a right angle (90 degrees)" ;
    rdfs:subClassOf dbpedia:Triangle .
