@prefix rdf: <http://www.w3.org/1999/02/22-rdf-syntax-ns#> .
@prefix rdfs: <http://www.w3.org/2000/01/rdf-schema#> .
@prefix xsd: <http://www.w3.org/2001/XMLSchema#> .
@prefix time: <http://www.w3.org/2006/time#> .
time:TemporalEntity a rdfs:Class ;
  rdfs:label "Temporal Entity" ;
  rdfs:comment "The abstract superclass of Temporal Positions and Temporal Intervals, all of which can be associated with numbers in several ways" .
time:TemporalPosition a rdfs:Class ;
  rdfs:subClassOf time:TemporalEntity ;
  rdfs:label "Temporal Position" ;
  rdfs:comment "An abstract reference to a position within a temporal coordinate system" .
time:TemporalInterval a rdfs:Class ;
  rdfs:subClassOf time:TemporalEntity ;
  rdfs:label "Temporal Interval" ;
  rdfs:comment "An interval of time that is bounded by two instants" .
time:inXSDDateTimeStamp a rdf:Property ;
  rdfs:domain time:TemporalPosition ;
  rdfs:range xsd:dateTimeStamp ;
  rdfs:label "in XSD DateTime Stamp" ;
  rdfs:comment "Connects a temporal position with a dateTimeStamp as defined in XML Schema" .
time:hasBeginning a rdf:Property ;
  rdfs:domain time:TemporalInterval ;
  rdfs:range time:TemporalPosition ;
  rdfs:label "has Beginning" ;
  rdfs:comment "The temporal interval has the specified temporal position as its beginning" .
time:hasEnd a rdf:Property ;
  rdfs:domain time:TemporalInterval ;
  rdfs:range time:TemporalPosition ;
  rdfs:label "has End" ;
  rdfs:comment "The temporal interval has the specified temporal position as its end" .
