@prefix rdf: <http://www.w3.org/1999/02/22-rdf-syntax-ns#> .
@prefix rdfs: <http://www.w3.org/2000/01/rdf-schema#> .
@prefix ow: <http://www.myontology.com/ontology#> .
ow:Information a rdfs:Class ;
  rdfs:label "Information" ;
  rdfs:comment "This class is meant to model any form of data or information." .
ow:hasInformation a rdf:Property ;
  rdfs:label "hasInformation" ;
  rdfs:range ow:Information ;
  rdfs:comment "Property stating that a specific entity has some information." .
ow:relatedInformation a rdf:Property ;
  rdfs:label "relatedInformation" ;
  rdfs:domain ow:Information ;
  rdfs:range ow:Information ;
  rdfs:comment "Property stating that one piece of information is related to another." .
