@prefix : <http://www.example.org/#> .
@prefix rdf: <http://www.w3.org/1999/02/22-rdf-syntax-ns#> .
@prefix rdfs: <http://www.w3.org/2000/01/rdf-schema#> .
@prefix owl: <http://www.w3.org/2002/07/owl#> .
:Eye rdf:type owl:Class ;
    rdfs:label "Eye"@en ;
    rdfs:comment "The organ of sight"@en ;
    rdfs:subClassOf <http://www.example.org/#Organ> ;
    :hasPart :Cornea ;
    :hasPart :Iris ;
    :hasPart :Lens ;
    :hasPart :Retina .
:Cornea rdf:type owl:Class ;
    rdfs:label "Cornea"@en ;
    rdfs:comment "The transparent layer forming the front of the eye."@en ;
    rdfs:subClassOf :Eye .
:Iris rdf:type owl:Class ;
    rdfs:label "Iris"@en ;
    rdfs:comment "The thin, circular structure in the eye, responsible for controlling the diameter and size of the pupil."@en ;
    rdfs:subClassOf :Eye .
:Lens rdf:type owl:Class ;
    rdfs:label "Lens"@en ;
    rdfs:comment "The transparent elastic structure in the eye that helps to control the amount of light reaching the retina."@en ;
    rdfs:subClassOf :Eye .
:Retina rdf:type owl:Class ;
    rdfs:label "Retina"@en ;
    rdfs:comment "The light-sensitive layer of tissue at the back of the inner eye that captures visual information."@en ;
    rdfs:subClassOf :Eye .
