@prefix rdfs: <http://www.w3.org/2000/01/rdf-schema#> .
@prefix game: <http://example.org/ontology/game#> .
game:Game a rdfs:Class ;
    rdfs:label "Game" ;
    rdfs:comment "A structured form of play, usually undertaken for entertainment or fun." .
game:VideoGame a rdfs:Class ;
    rdfs:label "Video Game" ;
    rdfs:comment "Electronic game that involves interaction with a user interface to generate visual feedback on a video device." ;
    rdfs:subClassOf game:Game .
game:BoardGame a rdfs:Class ;
    rdfs:label "Board Game" ;
    rdfs:comment "Game that involves counters or pieces moved or placed on a pre-marked surface or 'board', according to a set of rules." ;
    rdfs:subClassOf game:Game .
game:CardGame a rdfs:Class ;
    rdfs:label "Card Game" ;
    rdfs:comment "Any game using playing cards as the primary device with which the game is played." ;
    rdfs:subClassOf game:Game .
game:rule rdfs:Class ;
    rdfs:label "Game rule" ;
    rdfs:comment "Regulations to which the players must agree to follow for a game." .
game:genre rdfs:Class ;
    rdfs:label "Game genre" ;
    rdfs:comment "Specific category of games related by similar gameplay characteristics." .
game:hasRule a rdfs:Property ;
    rdfs:label "has rule" ;
    rdfs:domain game:Game ;
    rdfs:range game:rule ;
    rdfs:comment "Property that links a game to its rules." .
game:hasGenre a rdfs:Property ;
    rdfs:label "has genre" ;
    rdfs:domain game:Game ;
    rdfs:range game:genre ;
    rdfs:comment "Property that links a game to its genre." .
