@prefix rdf: <http://www.w3.org/1999/02/22-rdf-syntax-ns#> .
@prefix owl: <http://www.w3.org/2002/07/owl#> .
@prefix xsd: <http://www.w3.org/2001/XMLSchema#> .
@prefix rdfs: <http://www.w3.org/2000/01/rdf-schema#> .
@prefix face: <http://www.example.org/ontology/face#> .
face:     rdf:type owl:Ontology ;
    rdfs:comment "An ontology for the face."@en ;
    rdfs:label "Face Ontology"@en .
face:Face    rdf:type owl:Class ;
    rdfs:label "Face"@en ;
    rdfs:comment "A class representing the human face."@en .
    face:Eyebrow    rdf:type owl:Class ;
    rdfs:label "Eyebrow"@en ;
    rdfs:comment "Defines the part of the face above the eye"@en ;
    rdfs:subClassOf face:Face;
    face:Eye    rdf:type owl:Class ;
    rdfs:label "Eye"@en ;
    rdfs:comment "Defines the visual organ in humans and animals residing on the face"@en ;
    rdfs:subClassOf face:Face.face:Nose    rdf:type owl:Class ;
    rdfs:label "Nose"@en ;
    rdfs:comment "Defines the central part of the face used for smelling and breathing"@en ;
    rdfs:subClassOf face:Face.  face:Ear    rdf:type owl:Class ;
    rdfs:label "Ear"@en ;
    rdfs:comment "Defines the organ of hearing and balance residing on the side of the face"@en ;
    rdfs:subClassOf face:Face.face:Mouth    rdf:type owl:Class ;
    rdfs:label "Mouth"@en ;
    rdfs:comment "Defines the oral part of the face used for eating, speaking, and expressing emotions"@en ;
    rdfs:subClassOf face:Face.face:hasFeature    rdf:type owl:ObjectProperty ;
    rdfs:domain face:Face ;
    rdfs:range face:Eye, face:Ear, face:Mouth, face:Nose, face:Eyebrow ;
    rdfs:label "has feature"@en ;
    rdfs:comment "Defines the property that a face has an eye, ear, mouth, nose or eyebrow"@en .
