@prefix rdf: <http://www.w3.org/1999/02/22-rdf-syntax-ns#> .
@prefix rdfs: <http://www.w3.org/2000/01/rdf-schema#> .
@prefix foaf: <http://xmlns.com/foaf/0.1/> .
@prefix gov: <http://www.example.org/gov#> .
gov:Government     rdf:type rdfs:Class ;
    rdfs:label "Political Government" ;
    rdfs:comment "The organization, machinery, or agency, through which a political unit exercises authority and performs functions." .
gov:hasCountry     rdf:type rdf:Property ;
    rdfs:label "has country" ;
    rdfs:comment "The country a government rules over." ;
    rdfs:range foaf:Country .
gov:hasLeader     rdf:type rdf:Property ;
    rdfs:label "has leader" ;
    rdfs:comment "The leader of the government." ;
    rdfs:range foaf:Person .
gov:hasForm     rdf:type rdf:Property ;
    rdfs:label "has form" ;
    rdfs:comment "The form of government, e.g., democracy, oligarchy, monarchy etc." ;
    rdfs:range rdfs:Literal .
  gov:Political_Party    rdf:type rdfs:Class ;
    rdfs:label "Political Party" ;
    rdfs:comment "An organization that coordinates candidates to compete in a particular country's elections." .
gov:participatesIn     rdf:type rdf:Property ;
    rdfs:label "participates in" ;
    rdfs:comment "The government or political party's participation in a certain political process or event" ;
    rdfs:range rdfs:Resource .
gov:hasLaw     rdf:type rdf:Property ;
    rdfs:label "has law" ;
    rdfs:comment "The laws implemented by the government." ;
    rdfs:range gov:Law .
gov:Law    rdf:type rdfs:Class ;
    rdfs:label "Law" ;
    rdfs:comment "A system of rules adopted by the government." .
