@prefix rdf: <http://www.w3.org/1999/02/22-rdf-syntax-ns#> .
@prefix rdfs: <http://www.w3.org/2000/01/rdf-schema#> .
@prefix owl: <http://www.w3.org/2002/07/owl#> .
@prefix prg: <http://www.example.org/program#> .
### Ontology surrounding the concept of Program## Classesprg:Programm rdf:type owl:Class ;
   rdfs:comment "A series of coded software instructions to control the operation of a computer or other machine." ;
   rdfs:label "Program" .
prg:Software rdf:type owl:Class ;
   rdfs:comment "The programs and other operating information used by a computer." ;
   rdfs:label "Software" ;
   rdfs:subClassOf prg:Program .
prg:Script rdf:type owl:Class ;
   rdfs:comment "A program or sequence of instructions that is interpreted or carried out by another program rather than by the computer processor." ;
   rdfs:label "Script" ;
   rdfs:subClassOf prg:Program .
prg:Algorithm rdf:type owl:Class ;
   rdfs:comment "A process or set of rules to be followed in calculations or other problem-solving operations, especially by a computer." ;
   rdfs:label "Algorithm" ;
   rdfs:subClassOf prg:Program .
## Propertiesprg:isWrittenIn rdf:type owl:ObjectProperty ;
   rdfs:comment "Specifies the programming language that was used to write the program." ;
   rdfs:label "is written in" ;
   rdfs:domain prg:Program ;
   rdfs:range prg:ProgrammingLanguage .
prg:hasAuthor rdf:type owl:ObjectProperty ;
   rdfs:comment "Specifies the author of the program." ;
   rdfs:label "has author" ;
   rdfs:domain prg:Program ;
   rdfs:range prg:Programmer .
#######################################