@prefix rdf: <http://www.w3.org/1999/02/22-rdf-syntax-ns#> .
@prefix rdfs: <http://www.w3.org/2000/01/rdf-schema#> .
@prefix owl: <http://www.w3.org/2002/07/owl#> .
@prefix xsd: <http://www.w3.org/2001/XMLSchema#> .
@prefix foaf: <http://xmlns.com/foaf/0.1/> .
<#Friend> rdf:type owl:Class ;
          rdfs:subClassOf foaf:Person ;
          rdfs:label "Friend" ;
          rdfs:comment "The concept of a friend, i.e., an individual with whom one has a bond of mutual affection." .
<#hasFriend> rdf:type owl:ObjectProperty ;
             rdfs:domain <#Friend> ;
             rdfs:range <#Friend> ;
             rdfs:label "has friend" ;
             rdfs:comment "A property that describes a friendship relation between two friends." .
<#knowsSince> rdf:type owl:DatatypeProperty ;
              rdfs:domain <#hasFriend> ;
              rdfs:range xsd:date ;
              rdfs:label "knows since" ;
              rdfs:comment "A property that describes when two friends got to know each other." .
<#commonInterest> rdf:type owl:DatatypeProperty ;
                  rdfs:domain <#hasFriend> ;
                  rdfs:range xsd:string ;
                  rdfs:label "common interest" ;
                  rdfs:comment "A property that describes a common interest between two friends." .
