@prefix rdfs: <http://www.w3.org/2000/01/rdf-schema#> .
@prefix : <http://example.org/back#> .
:Back a rdfs:Class ;
  rdfs:label "Back" ;
  rdfs:comment "The body part on the opposite of the chest, between the neck and the tail in humans or animals" .
:Spine a rdfs:Class ;
  rdfs:subClassOf :Back ;
  rdfs:label "Spine" ;
  rdfs:comment "The column of bone and tissue extending from the base of the skull and enclosing the spinal cord, a part of back" .
:Muscles a rdfs:Class ;
  rdfs:subClassOf :Back ;
  rdfs:label "Muscles" ;
  rdfs:comment "Tissues in the back that can contract, producing movement or maintaining the position of parts of the body" .
:Nerves a rdfs:Class ;
  rdfs:subClassOf :Back ;
  rdfs:label "Nerves" ;
  rdfs:comment "A bundle of fibers that transmits impulses of sensation to the brain or spinal cord, and impulses from these to the muscles and organs" .
:BackPain a rdfs:Class ;
  rdfs:subClassOf :Back ;
  rdfs:label "Back Pain" ;
  rdfs:comment "Pain felt in the back that may come from the spine, muscles, nerves, or other structures in the back" .
:BackInjury a rdfs:Class ;
  rdfs:subClassOf :Back ;
  rdfs:label "Back Injury" ;
  rdfs:comment "Any type of harm or damage to the backbone or any part of the back" .
:UpperBack a rdfs:Class ;
  rdfs:subClassOf :Back ;
  rdfs:label "Upper Back" ;
  rdfs:comment "The region of the back ranging from the base of the neck to the bottom of the rib cage" .
:LowerBack a rdfs:Class ;
  rdfs:subClassOf :Back ;
  rdfs:label "Lower Back" ;
  rdfs:comment "The region of the back extending from the bottom of the rib cage to the tailbone" .
