@prefix owl: <http://www.w3.org/2002/07/owl#> .
@prefix rdfs: <http://www.w3.org/2000/01/rdf-schema#> .
@prefix rdf: <http://www.w3.org/1999/02/22-rdf-syntax-ns#> .
@prefix xsd: <http://www.w3.org/2001/XMLSchema#> .
@prefix system: <http://example.org/system#> .
system:     a owl:Ontology ;
     rdfs:comment "A simple ontology model for System" .
system:System     a owl:Class ;
    rdfs:label "System" ;
    rdfs:comment "A System is a set of interacting or interdependent components forming an integrated whole" .
system:Subsystem    a owl:Class ;
    rdfs:label "Subsystem" ;
    rdfs:comment "A Subsystem is a self-contained system within a larger system." ;
    rdfs:subClassOf system:System .
system:hasComponent    a owl:ObjectProperty ;
    rdfs:label "has component" ;
    rdfs:comment "Relates a system to its components or parts" ;
    rdfs:domain system:System ;
    rdfs:range system:System .
system:hasFunction    a owl:DatatypeProperty ;
    rdfs:label "has function" ;
    rdfs:comment "Relates a system to a description of its function or purpose" ;
    rdfs:domain system:System ;
    rdfs:range xsd:string .
