@prefix rdf: <http://www.w3.org/1999/02/22-rdf-syntax-ns#> .
@prefix rdfs: <http://www.w3.org/2000/01/rdf-schema#> .
@prefix owl: <http://www.w3.org/2002/07/owl#> .
@prefix xsd: <http://www.w3.org/2001/XMLSchema#> .
@prefix air: <http://www.example.org/air#> .
air: a owl:Ontology ;
    rdfs:comment "An ontology about Air"@en .
air:Air a owl:Class ;
    rdfs:comment "The substance that forms the Earth's atmosphere and that we breathe"@en ;
    rdfs:label "Air"@en .
air:hasTemperature a owl:ObjectProperty ;
    rdfs:domain air:Air ;
    rdfs:range xsd:float ;
    rdfs:comment "The property that determines the temperature of the air"@en ;
    rdfs:label "hasTemperature"@en .
 air:hasPressure a owl:ObjectProperty ;
    rdfs:domain air:Air ;
    rdfs:range xsd:float ;
    rdfs:comment "The property that determines the pressure of the air"@en ;
    rdfs:label "hasPressure"@en .
air:hasHumidity a owl:ObjectProperty ;
    rdfs:domain air:Air ;
    rdfs:range xsd:float ;
    rdfs:comment "The property that determines the amount of moisture in the air"@en ;
    rdfs:label "hasHumidity"@en .
air:hasPollutants a owl:ObjectProperty ;
    rdfs:domain air:Air ;
    rdfs:range xsd:string ;
    rdfs:comment "The property that determines the presence of harmful substances in the air"@en ;
    rdfs:label "hasPollutants"@en .
air:isComposedOf a owl:ObjectProperty ;
    rdfs:domain air:Air ;
    rdfs:range xsd:string ;
    rdfs:comment "The property that determines what gases the air is composed of"@en ;
    rdfs:label "isComposedOf"@en .
 air:isInArea a owl:ObjectProperty ;
    rdfs:domain air:Air ;
    rdfs:range xsd:string ;
    rdfs:comment "The property that determines the area where the air is"@en ;
    rdfs:label "isInArea"@en .
