@prefix xsd: <http://www.w3.org/2001/XMLSchema#> .
@prefix rdf: <http://www.w3.org/1999/02/22-rdf-syntax-ns#> .
@prefix rdfs: <http://www.w3.org/2000/01/rdf-schema#> .
@prefix owl: <http://www.w3.org/2002/07/owl#> .
@prefix issue: <http://www.specific_domain.com/ontology/issue/> .
issue:Issue rdf:type rdfs:Class ;
    rdfs:label "Issue" ;
    rdfs:comment "Represents any issue, problem or situation that needs to be addressed, solved or managed." .
issue:hasID rdf:type rdf:Property ;
    rdfs:label "has ID" ;
    rdfs:comment "The unique identifier of the Issue" ;
    rdfs:domain issue:Issue ;
    rdfs:range xsd:string .
issue:hasDescription rdf:type rdf:Property ;
    rdfs:label "has description" ;
    rdfs:comment "The detailed explanation or description of the Issue." ;
    rdfs:domain issue:Issue ;
    rdfs:range xsd:string .
issue:hasStatus rdf:type rdf:Property ;
    rdfs:label "has status" ;
    rdfs:comment "Indicates the current status of the issue (open, closed, in progress, etc.)" ;
    rdfs:domain issue:Issue ;
    rdfs:range issue:Status .
issue:Status rdf:type rdfs:Class ;
    rdfs:label "Status" ;
    rdfs:comment "Represents the current status of an issue." .
issue:isOpen rdf:type issue:Status ;
    rdfs:label "Is Open" ;
    rdfs:comment "Indicates the issue is open and needs action." .
issue:isClosed rdf:type issue:Status ;
    rdfs:label "Is Closed" ;
    rdfs:comment "Indicates the issue has been resolved or actioned." .
issue:isInProgress rdf:type issue:Status ;
    rdfs:label "Is In Progress" ;
    rdfs:comment "Indicates the issue is currently being actioned or resolved." .
