@prefix : <http://example.com/> .
@prefix rdf: <http://www.w3.org/1999/02/22-rdf-syntax-ns#> .
@prefix rdfs: <http://www.w3.org/2000/01/rdf-schema#> .
@prefix owl: <http://www.w3.org/2002/07/owl#> .
:Other     rdf:type owl:Class ;
    rdfs:label "Other"@en ;
    rdfs:comment "This represents the category of individuals or entities that are not included in the primary classification or category"@en.:Individual    rdf:type owl:Class ;
    rdfs:subClassOf :Other;
    rdfs:label "Individual"@en ;
    rdfs:comment "This represents a person who falls under the category of Others"@en .
:Entity    rdf:type owl:Class ;
    rdfs:subClassOf :Other;
    rdfs:label "Entity"@en ;
    rdfs:comment "This represents a thing (like an organization) that falls under the category of Others"@en .
:hasAttribute     rdf:type owl:ObjectProperty ;
    rdfs:domain :Other ;
    rdfs:range :Attribute;
    rdfs:label "hasAttribute"@en ;
    rdfs:comment "Property showing the attributes belonging to Others"@en .
:Attribute     rdf:type owl:Class ;
    rdfs:label "Attribute"@en ;
    rdfs:comment "This represents the attributes or properties belonging to Others"@en .
