@prefix rdf: <http://www.w3.org/1999/02/22-rdf-syntax-ns#> .
@prefix rdfs: <http://www.w3.org/2000/01/rdf-schema#> .
@prefix xsd: <http://www.w3.org/2001/XMLSchema#> .
@prefix owl: <http://www.w3.org/2002/07/owl#> .
@prefix ppl: <http://example.org/people#> .
ppl:Person a owl:Class ;
    rdfs:subClassOf owl:Thing ;
    rdfs:label "Person"@en ;
    rdfs:comment "Represents a human being, regardless of their age, gender, nationality, profession, religion, etc."@en .
ppl:Friend a owl:Class ;
    rdfs:subClassOf ppl:Person ;
    rdfs:label "Friend"@en ;
    rdfs:comment "A Person who is known well to another and is regarded with liking, affection, and loyalty."@en .
ppl:hasFriend a owl:ObjectProperty ;
    rdfs:domain ppl:Person ;
    rdfs:range ppl:Friend ;
    rdfs:label "has friend"@en ;
    rdfs:comment "Holds between a person and another person who the former knows well and regards with affection and trust."@en .
ppl:knowsSince a owl:DatatypeProperty ;
    rdfs:domain ppl:hasFriend ;
    rdfs:range xsd:date ;
    rdfs:label "knows since"@en ;
    rdfs:comment "The date since when two persons know each other and have a friendship relationship."@en .
