@prefix rdf: <http://www.w3.org/1999/02/22-rdf-syntax-ns#> .
@prefix rdfs: <http://www.w3.org/2000/01/rdf-schema#> .
@prefix xsd: <http://www.w3.org/2001/XMLSchema#> .
@prefix home: <http://example.com/home#> .
#:Homehome:Home rdf:type rdfs:Class ;
    rdfs:comment "A place where an individual or family lives" .
#:Roomhome:Room rdf:type rdfs:Class ;
    rdfs:subClassOf home:Home ;
    rdfs:comment "A part or division of a building enclosed by walls, floor, and ceiling" .
#:Kitchenhome:Kitchen rdf:type rdfs:Class ;
    rdfs:subClassOf home:Room ;
    rdfs:comment "A room used for cooking and food preparation" .
#:Bedroomhome:Bedroom rdf:type rdfs:Class ;
    rdfs:subClassOf home:Room ;
    rdfs:comment "A room in a house where people sleep" .
#:Bathroomhome:Bathroom rdf:type rdfs:Class ;
    rdfs:subClassOf home:Room ;
    rdfs:comment "A room containing a bath or shower and typically also a washbasin and a toilet" .
#:LivingRoomhome:LivingRoom rdf:type rdfs:Class ;
    rdfs:subClassOf home:Room ;
    rdfs:comment "A room in a house for general and informal everyday use" .
#:hasRoomhome:hasRoom rdf:type rdf:Property ;
    rdfs:domain home:Home;
    rdfs:range home:Room;
    rdfs:comment "Property to link a Home to its Rooms" .
#:hasFurniturehome:hasFurniture rdf:type rdf:Property ;
    rdfs:domain home:Room ;
    rdfs:range rdfs:Resource ;
    rdfs:comment "Property to link a Room to its Furniture" .
#:Furniturehome:Furniture rdf:type rdfs:Class ;
    rdfs:comment "Movable objects intended to support human activities" .
#:Tablehome:Table rdf:type home:Furniture ;
    rdfs:comment "An item of Furniture with a flat top and one or more legs" .
#:Chairhome:Chair rdf:type home:Furniture ;
    rdfs:comment "A seat for one person, with a support for the back" .
#:Bedhome:Bed rdf:type home:Furniture ;
    rdfs:comment "A piece of Furniture upon which or within which a person sleeps, rests, or stays when not well." .
#:Couchhome:Couch rdf:type home:Furniture ;
    rdfs:comment "A large piece of Furniture that can be sat on by several people" .
#:Cupboardhome:Cupboard rdf:type home:Furniture ;
    rdfs:comment "A piece of Furniture with shelves that are used for storing items, usually has doors" .
#:Refrigeratorhome:Refrigerator rdf:type home:Furniture ;
    rdfs:comment "A large container that uses electricity to keep food cold." .
