@prefix rdf: <http://www.w3.org/1999/02/22-rdf-syntax-ns#> .
@prefix owl: <http://www.w3.org/2002/07/owl#> .
@prefix xsd: <http://www.w3.org/2001/XMLSchema#> .
@prefix rdfs: <http://www.w3.org/2000/01/rdf-schema#> .
@prefix power: <http://example.org/power#> .
power:     rdf:type owl:Ontology ;
    rdfs:comment "Ontology about the concept of Power" .
power:Power     rdf:type owl:Class ;
    rdfs:label "The concept of Power" ;
    rdfs:comment "The capacity or ability to direct or influence the behavior of others or the course of events".
power:PhysicalPower     rdf:type owl:Class ;
    rdfs:subClassOf power:Power ;
    rdfs:label "Physical Power" ;
    rdfs:comment "The capacity to do work or cause physical change".
power:SocialPower     rdf:type owl:Class ;
    rdfs:subClassOf power:Power ;
    rdfs:label "Social Power" ;
    rdfs:comment "The degree to which an individual or organization can influence others".
power:PoliticalPower     rdf:type owl:Class ;
    rdfs:subClassOf power:Power ;
    rdfs:label "Political Power" ;
    rdfs:comment "The capacity to influence or control the behavior of people, typically through governance".
power:hasPower     rdf:type owl:ObjectProperty ;
    rdfs:domain owl:Thing ;
    rdfs:range power:Power ;
    rdfs:label "has power" ;
    rdfs:comment "An object property to show that a person or organization possesses power" .
 power:amountOfPower     rdf:type owl:DatatypeProperty ;
      rdfs:domain power:Power ;
     rdfs:range xsd:integer ;
    rdfs:label "amount of power" ;
    rdfs:comment "A data property to describe the quantity or intensity of power" .
