@prefix rdf: <http://www.w3.org/1999/02/22-rdf-syntax-ns#> .
@prefix rdfs: <http://www.w3.org/2000/01/rdf-schema#> .
@prefix health: <http://www.example.com/health#> .
health:Disease rdf:type rdfs:Class ;
    rdfs:label "Disease" ;
    rdfs:comment "Disease is an abnormal condition affecting the body of an organism" .
    health:Symptom rdf:type rdfs:Class ;
    rdfs:label "Symptom" ;
    rdfs:comment "Symptoms are signs or signals of disease or disorder".
health:hasSymptom rdf:type rdf:Property;
    rdfs:label "has symptom";
    rdfs:domain health:Disease;
    rdfs:range health:Symptom;
    rdfs:comment "Relates a disease to its symptoms".
health:Treatment rdf:type rdfs:Class;
    rdfs:label "Treatment";
    rdfs:comment "Medical treatment is a procedure used to cure, manage or prevent a disease".
health:hasTreatment rdf:type rdf:Property;
    rdfs:label "has treatment";
    rdfs:domain health:Disease;
    rdfs:range health:Treatment;
    rdfs:comment "Relates a disease to its treatment".
    health:HealthCareProfessional rdf:type rdfs:Class;
    rdfs:label "HealthCareProfessional";
    rdfs:comment "Healthcare professional is a person who is qualified and licensed to provide health care services".
