@prefix rdf: <http://www.w3.org/1999/02/22-rdf-syntax-ns#> .
@prefix rdfs: <http://www.w3.org/2000/01/rdf-schema#> .
@prefix xsd: <http://www.w3.org/2001/XMLSchema#> .
@prefix owl: <http://www.w3.org/2002/07/owl#> .
@prefix my: <http://www.example.org/myOntology#> .
my:System rdf:type owl:Class ;
   rdfs:comment "A set of interacting or interdependent component parts forming a complex whole."@en .
my:hasComponent rdf:type owl:ObjectProperty ;
  rdfs:domain my:System ;
  rdfs:range my:Component ;
  rdfs:comment "The property that connects a system with its components."@en .
my:Component rdf:type owl:Class ;
  rdfs:comment "A part or element of a larger whole, especially a part of a machine or vehicle."@en .
my:isPartOf rdf:type owl:ObjectProperty ;
  rdfs:domain my:Component ;
  rdfs:range my:System ;
  rdfs:comment "This property connects a component to the system that it forms part of."@en .
