@prefix rdf: <http://www.w3.org/1999/02/22-rdf-syntax-ns#> .
@prefix rdfs: <http://www.w3.org/2000/01/rdf-schema#> .
@prefix bus: <http://www.example.org/business#> .
bus:Company   rdf:type rdfs:Class ;
  rdfs:comment "An organization engaged in commercial, industrial, or professional activities."@en ;
.bus:Employee  rdf:type rdfs:Class ;
  rdfs:comment "An individual who works part-time or full-time under a contract of employment."@en ;
.bus:hasEmployee   rdf:type rdf:Property ;
  rdfs:domain bus:Company ;
  rdfs:range bus:Employee ;
  rdfs:comment "Relates a company to its employees."@en ;
.bus:Product   rdf:type rdfs:Class ;
  rdfs:comment "An article or substance manufactured or refined for sale, created by a company."@en ;
.bus:produces   rdf:type rdf:Property ;
  rdfs:domain bus:Company ;
  rdfs:range bus:Product ;
  rdfs:comment "Relates a company to its produced products."@en ;
.bus:Customer   rdf:type rdfs:Class ;
  rdfs:comment "A person or organisation that buys goods or services from a store or business."@en ;
.bus:buysFrom   rdf:type rdf:Property ;
  rdfs:domain bus:Customer ;
  rdfs:range bus:Company ;
  rdfs:comment "Relates a customer to the companies they purchase from."@en ;
.bus:Market  rdf:type rdfs:Class ;
  rdfs:comment "Area of economic activity in which buyers and sellers come into contact to trade goods and services."@en ;
.bus:operatesIn  rdf:type rdf:Property ;
  rdfs:domain bus:Company ;
  rdfs:range bus:Market ;
  rdfs:comment "Relates a company to the markets it operates in."@en ;
  .
