@prefix xsd: <http://www.w3.org/2001/XMLSchema#> .
@prefix : <http://example.org/time#> .
:Minute a rdfs:Class ;
    rdfs:comment "A unit of time equivalent to sixty seconds or 1/60th of an hour."@en ;
    rdfs:label "Minute"@en .
:TimePeriod a rdfs:Class ;
    rdfs:label "Time Period"@en ;
    rdfs:comment "A period of time that can be described in units like seconds, minutes, hours, etc."@en ;
    rdfs:subClassOf [      a owl:Restriction ;
      owl:onProperty :hasDuration ;
      owl:someValuesFrom :Minute    ] .
:hasDuration a rdf:Property ;
    rdfs:range :Minute ;
    rdfs:domain :TimePeriod ;
    rdfs:label "has duration"@en ;
    rdfs:comment "A property that links a time period to its duration in minutes."@en .
:meetingExample a :TimePeriod ;
    :hasDuration "60"^^xsd:integer .
