@prefix rdf: <http://www.w3.org/1999/02/22-rdf-syntax-ns#> .
@prefix rdfs: <http://www.w3.org/2000/01/rdf-schema#> .
@prefix owl: <http://www.w3.org/2002/07/owl#> .
@prefix case: <http://www.example.org/ontology/case#> .
case:Case  rdf:type rdfs:Class ;
  rdfs:label "Case"@en ;
  rdfs:comment "A general concept to describe a situation or instance of something being processed or considered, often in a legal, medical or other disciplinary context"@en ;
.case:hasCaseID  rdf:type owl:DatatypeProperty ;
  rdfs:label "has case ID"@en ;
  rdfs:comment "A unique identifier for a case"@en ;
  rdfs:domain case:Case ;
  rdfs:range rdf:XMLLiteral ;
.case:hasCaseStatus  rdf:type owl:DatatypeProperty ;
  rdfs:label "has case status"@en ;
  rdfs:comment "The current status or stage of case"@en ;
  rdfs:domain case:Case ;
  rdfs:range rdfs:Literal ;
.case:hasCaseType  rdf:type owl:ObjectProperty ;
  rdfs:label "has case type"@en ;
  rdfs:comment "The type of the case instance, such as legal, medical, etc"@en ;
  rdfs:domain case:Case ;
  rdfs:range case:CaseType ;
.case:CaseType  rdf:type rdfs:Class ;
  rdfs:label "Case Type"@en ;
  rdfs:comment "A classification for the type of case, such as legal, medical, etc"@en ;
.case:associatedWith  rdf:type owl:ObjectProperty ;
  rdfs:label "is associated with"@en ;
  rdfs:comment "A relation to denote the association of case to an entity, may be a person, organization or any other object of interest"@en ;
  rdfs:domain case:Case ;
  rdfs:range rdfs:Resource ;
.