@prefix rdf: <http://www.w3.org/1999/02/22-rdf-syntax-ns#> .
@prefix rdfs: <http://www.w3.org/2000/01/rdf-schema#> .
@prefix owl: <http://www.w3.org/2002/07/owl#> .
@prefix : <http://example.org/> .
:Door a owl:Class ;
    rdfs:label "Door"@en ;
    rdfs:comment "A door is a hinged or otherwise movable barrier that allows ingress into and egress from an enclosure. The opening in the wall can be referred to as a portal. The 'door's' essential and primary purpose is to provide security by controlling access to the portal (doorway)."@en ;
    .
:hasMaterial a owl:ObjectProperty ;
    rdfs:label "has material"@en ;
    rdfs:comment "Property that represents the material a door is made of"@en ;
    rdfs:domain :Door ;
    rdfs:range :Material .
    :Material a owl:Class ;
    rdfs:label "Material"@en ;
    rdfs:comment "Substance or substances out of which a thing is or can be made."@en ;
    .
:isOpenedBy a owl:ObjectProperty ;
    rdfs:label "is opened by"@en ;
    rdfs:comment "Property that signifies what can open a door"@en ;
    rdfs:domain :Door ;
    rdfs:range :Key .
    :Key a owl:Class ;
    rdfs:label "Key"@en ;
    rdfs:comment "A small piece of shaped metal with incisions cut to fit the wards of a particular lock, and that is inserted into a lock and turned to open or close it."@en ;
    .
