@prefix : <http://example.org#> .
@prefix rdf: <http://www.w3.org/1999/02/22-rdf-syntax-ns#> .
@prefix owl: <http://www.w3.org/2002/07/owl#> .
@prefix rdfs: <http://www.w3.org/2000/01/rdf-schema#> .
### Definition of law:Law rdf:type owl:Class ;
    rdfs:comment "A system of rules created by a social or governmental institution" ;
    rdfs:label "Law" .
### Properties
 of law:hasJurisdiction rdf:type owl:ObjectProperty ;
    rdfs:label "has jurisdiction" ;
    rdfs:comment "The jurisdiction, typically a country or state, where the law is legislated." ;
    rdfs:domain :Law .
:hasTopic rdf:type owl:ObjectProperty ;
    rdfs:label "has topic" ;
    rdfs:comment "The topic or field that the law covers, such as criminal law, civil law, contract law, etc." ;
    rdfs:domain :Law .
:hasExplanation rdf:type owl:DatatypeProperty ;
    rdfs:label "has explanation" ;
    rdfs:domain :Law ;
    rdfs:range xsd:string .
### Instances of law:CriminalLaw rdf:type :Law ;
    :hasJurisdiction "USA" ;
    :hasTopic "Criminal Law" ;
    :hasExplanation "A system of law concerned with punishment of individuals who commit crimes." .
