@prefix rdf: <http://www.w3.org/1999/02/22-rdf-syntax-ns#> .
@prefix rdfs: <http://www.w3.org/2000/01/rdf-schema#> .
@prefix xsd: <http://www.w3.org/2001/XMLSchema#> .
@prefix way: <http://example.org/way/> .
way:     a rdfs:Class ;
    rdfs:label "Way"@en ;
    rdfs:comment "A Class representing all kinds of ways or paths for traversal on land, air or water."@en .
way:hasLength    a rdf:Property ;
    rdfs:label "has length"@en ;
    rdfs:domain way: ;
    rdfs:range xsd:integer .
way:hasSourceType    a rdf:Property ;
    rdfs:label "has source type"@en ;
    rdfs:domain way: ;
    rdfs:range rdfs:Resource .
way:hasDestinationType    a rdf:Property ;
    rdfs:label "has destination type"@en ;
    rdfs:domain way: ;
    rdfs:range rdfs:Resource .
way:hasMedium    a rdf:Property ;
    rdfs:label "has medium"@en ;
    rdfs:domain way: ;
    rdfs:range rdfs:Resource .
way:Road     a rdfs:Class ;
    rdfs:subClassOf way: ;
    rdfs:label "Road"@en ;
    rdfs:comment "A type of way specific to land travel, usually paved and strict for vehicle use."@en .
way:Airway     a rdfs:Class ;
    rdfs:subClassOf way: ;
    rdfs:label "Airway"@en ;
    rdfs:comment "A type of way specific to air travel, a defined corridor that aircrafts follow."@en .
way:Waterway     a rdfs:Class ;
    rdfs:subClassOf way: ;
    rdfs:label "Waterway"@en ;
    rdfs:comment "A type of way specific to water travel, a navigable route for traveling and transport over water."@en .
