@prefix rdf: <http://www.w3.org/1999/02/22-rdf-syntax-ns#> .
@prefix rdfs: <http://www.w3.org/2000/01/rdf-schema#> .
@prefix owl: <http://www.w3.org/2002/07/owl#> .
@prefix xsd: <http://www.w3.org/2001/XMLSchema#> .
@prefix law: <http://www.example.org/law#> .
law:Law rdfs:subClassOf rdf:Property ;
  rdfs:label "Law"@en ;
  rdfs:comment "Legislation passed by a competent authority establishing some course of conduct"@en .
law:CriminalLaw rdfs:subClassOf law:Law ;
  rdfs:label "Criminal Law"@en ;
  rdfs:comment "The body of law that relates to crime"@en .
law:CivilLaw rdfs:subClassOf law:Law ;
  rdfs:label "Civil Law"@en ;
  rdfs:comment "The body of law that relates to private relations between members of a community"@en ;
law:ConstitutionalLaw rdfs:subClassOf law:Law ;
  rdfs:label "Constitutional Law"@en ;
  rdfs:comment "The body of law that defines the relationship between different entities within a nation, most commonly the judiciary, the executive and the legislature bodies"@en ;
law:Statute rdfs:subClassOf rdf:Property ;
  rdfs:label "Statute"@en ;
  rdfs:comment "A written law passed by a legislative body"@en .
law:Case rdfs:subClassOf rdf:Property ;
  rdfs:label "Case"@en ;
  rdfs:comment "A legal action, cause, suit, or controversy, at law or in equity"@en .
law:Lawyer rdfs:subClassOf rdf:Property ;
  rdfs:label "Lawyer"@en ;
  rdfs:comment "A person who practices or studies law;
 an attorney or a counselor"@en .
law:Judge rdfs:subClassOf rdf:Property ;
  rdfs:label "Judge"@en ;
  rdfs:comment "A public official appointed to decide cases in a court of law"@en .
