@prefix foaf: <http://xmlns.com/foaf/0.1/> .
@prefix rdfs: <http://www.w3.org/2000/01/rdf-schema#> .
@prefix rdf: <http://www.w3.org/1999/02/22-rdf-syntax-ns#> .
@prefix xsd: <http://www.w3.org/2001/XMLSchema#> .
@prefix money: <http://www.example.org/money#> .
money:Currency  rdf:type rdfs:Class ;
  rdfs:label "Currency"@en ;
  rdfs:comment "An entity which represents a system of money in common use, especially in a nation."@en.money:CurrencyCode  rdf:type rdfs:Class ;
  rdfs:label "Currency Code"@en ;
  rdfs:comment "An abbreviated form of currency used in financial transaction and representation"@en.money:hasCurrencyCode  rdf:type rdf:Property ;
  rdfs:label "has currency code"@en ;
  rdfs:comment "The property which represents the currency code of a given currency"@en ;
  rdfs:domain money:Currency ;
  rdfs:range money:CurrencyCode .
money:hasValue  rdf:type rdf:Property ;
  rdfs:label "has value"@en ;
  rdfs:comment "The property which represents the nominal value of a currency"@en ;
  rdfs:domain money:Currency ;
  rdfs:range xsd:decimal .
money:Banknote  rdf:type rdfs:Class ;
  rdfs:label "Banknote"@en ;
  rdfs:comment "A type of negotiable instrument known as a promissory note, made by a bank, payable to the bearer on demand."@en;
  rdfs:subClassOf money:Currency .
money:Coin  rdf:type rdfs:Class ;
  rdfs:label "Coin"@en ;
  rdfs:comment "A small, flat, and usually round piece of metal issued by a government as a form of money."@en;
  rdfs:subClassOf money:Currency .
