@prefix : <http://www.example.com/money#> .
@prefix rdfs: <http://www.w3.org/2000/01/rdf-schema#> .
@prefix owl: <http://www.w3.org/2002/07/owl#> .
:Currency a rdfs:Class ;
    rdfs:comment "A system of money in common use, especially for people in a nation" .
:ExchangeRate a rdfs:Class ;
    rdfs:comment "The value of one currency for the purpose of conversion to another." .
:Bank a rdfs:Class ;
    rdfs:comment "A financial institution that accepts deposits from the public and creates credit." .
:intersectionCurrency a owl:Class ;
    owl:intersectionOf (        :Currency        :Bank    ) ;
    rdfs:comment "The intersection of Currency and Bank." .
:Bank rdfs:subClassOf :Currency ;
    rdfs:comment "A Bank is also considered as a sub-class of Currency".
:Currency rdfs:subClassOf :ExchangeRate ;
    rdfs:comment "Currency is considered as a sub-class of Exchange rate".
:hasCurrency a rdf:Property ;
    rdfs:domain :Bank ;
    rdfs:range :Currency ;
    rdfs:comment "A property indicating the specific currency a bank deals with".
:hasExchangeRate a rdf:Property ;
    rdfs:domain :Bank ;
    rdfs:range :ExchangeRate ;
    rdfs:comment "A property indicating the specific exchange rate a bank offers".
    :hasBank a rdf:Property ;
    rdfs:domain :Currency ;
    rdfs:range :Bank ;
    rdfs:comment "A property indicating the specific bank that deals with specific currency".
