@prefix rdf: <http://www.w3.org/1999/02/22-rdf-syntax-ns#> .
@prefix rdfs: <http://www.w3.org/2000/01/rdf-schema#> .
@prefix xsd: <http://www.w3.org/2001/XMLSchema#> .
@prefix owl: <http://www.w3.org/2002/07/owl#> .
@prefix money: <http://example.com/ontology/money#> .
money:   rdf:type owl:Ontology ;
  rdfs:comment "An ontology about the concept of money" .
money:Money   rdf:type owl:Class ;
  rdfs:comment "A medium that can be exchanged for goods and services and is used as a measure of their values on the market, including but not limited to coin and paper money as well as demand deposits." .
money:hasCurrency  rdf:type owl:ObjectProperty ;
  rdfs:domain money:Money ;
  rdfs:range money:Currency ;
  rdfs:comment "The currency in which a given amount of money is denominated." .
money:hasValue  rdf:type owl:DatatypeProperty ;
  rdfs:domain money:Money ;
  rdfs:range xsd:float ;
  rdfs:comment "The numerical value of a given amount of money." .
money:Currency   rdf:type owl:Class ;
  rdfs:comment "A system of money (monetary units) in common use, especially for people in a nation." .
money:Currency rdfs:subClassOf   [ rdf:type owl:Restriction ;
    owl:onProperty money:hasCurrency ;
    owl:someValuesFrom [      rdf:type owl:Class ;
      owl:unionOf (         money:Coins        money:PaperMoney        money:DemandDeposits      ) ] ].money:Coins   rdf:type owl:Class ;
  rdfs:comment "Metallic forms of money." .
money:PaperMoney  rdf:type owl:Class ;
  rdfs:comment "Paper notes used as money." .
money:DemandDeposits  rdf:type owl:Class ;
  rdfs:comment "Deposit account balances from which withdrawals can be made on demand." .
