@prefix : <http://example.org/money#> .
@prefix rdfs: <http://www.w3.org/2000/01/rdf-schema#> .
@prefix xsd: <http://www.w3.org/2001/XMLSchema#> .
:Money rdf:type rdfs:Class ;
        rdfs:label "Money"@en ;
       rdfs:comment "A medium of exchange for goods and services, which includes currency notes, coins, bank deposits."@en .
:Currency rdf:type rdfs:Class ;
           rdfs:label "Currency"@en ;
           rdfs:subClassOf :Money ;
          rdfs:comment "Physical or digital form of money that is used as a medium of exchange in a particular country or region."@en .
:DigitalCurrency rdf:type rdfs:Class ;
                  rdfs:label "Digital Currency"@en ;
                 rdfs:subClassOf :Currency ;
                 rdfs:comment "A type of currency that is non-physical and represented only in digital format."@en .
:Coin rdf:type rdfs:Class ;
       rdfs:label "Coin"@en ;
       rdfs:subClassOf :Currency ;
      rdfs:comment "Physical form of money, typically made of metal and minted by an sovereign authority."@en .
:BankDeposit rdf:type rdfs:Class ;
              rdfs:label "Bank Deposit"@en ;
              rdfs:subClassOf :Money ;
             rdfs:comment "A type of money that is placed into a banking institution for safekeeping."@en .
:hasValue rdf:type rdf:Property ;
          rdfs:label "has value"@en ;
          rdfs:comment "Property that indicates the value of the corresponding form of money."@en ;
          rdfs:range xsd:decimal .
 :hasCurrencyName rdf:type rdf:Property ;
                rdfs:label "has currency name"@en ;
                rdfs:comment "Property that indicates the name or type of the currency."@en ;
                rdfs:range xsd:string .
 :hasCountry rdf:type rdf:Property ;
            rdfs:label "has country"@en ;
            rdfs:comment "Property that indicates the country where the currency is used."@en ;
            rdfs:range xsd:string .
