@prefix : <http://example.org/#> .
@prefix rdf: <http://www.w3.org/1999/02/22-rdf-syntax-ns#> .
@prefix rdfs: <http://www.w3.org/2000/01/rdf-schema#> .
:Thing a rdfs:Class ;
  rdfs:label "Thing"@en ;
  rdfs:comment "A super-class to represent any thing or entity in the universe."@en ;
  rdfs:subClassOf rdfs:Resource .
:PhysicalObject a rdfs:Class ;
  rdfs:label "PhysicalObject"@en ;
  rdfs:comment "Physical objects that exist in physical space."@en ;
  rdfs:subClassOf :Thing .
:AbstractObject a rdfs:Class ;
  rdfs:label "AbstractObject"@en ;
  rdfs:comment "Objects that do not exist in physical space, but exist in conceptual space."@en ;
  rdfs:subClassOf :Thing .
  :Entity a rdfs:Class ;
  rdfs:label "Entity"@en ;
  rdfs:comment "A class to represent entities which could be physical or conceptual."@en ;
  rdfs:subClassOf :Thing .
