@prefix ex: <http://example.org/> .
@prefix rdf: <http://www.w3.org/1999/02/22-rdf-syntax-ns#> .
@prefix owl: <http://www.w3.org/2002/07/owl#> .
@prefix rdfs: <http://www.w3.org/2000/01/rdf-schema#> .
ex:Hand a owl:Class ;
  rdfs:label "Hand"@en ;
  rdfs:comment "A part of human body used to hold, move, touch and feel things"@en ;
  rdfs:subClassOf ex:BodyPart .
ex:hasHand a owl:ObjectProperty ;
  rdfs:label "has hand"@en ;
  rdfs:domain ex:Human ;
  rdfs:range ex:Hand .
ex:HandFunction a owl:Class ;
  rdfs:label "Hand function"@en ;
  rdfs:comment "The different functionalities a hand can provide (like holding, moving, touching and feeling things)"@en ;
  rdfs:subClassOf ex:Function .
ex:providesFunction a owl:ObjectProperty ;
  rdfs:label "provides function"@en ;
  rdfs:domain ex:Hand ;
  rdfs:range ex:HandFunction .
ex:Human a owl:Class ;
  rdfs:label "Human"@en ;
  rdfs:comment "A member of the Homo sapiens species, a branch of hominids"@en ;
  rdfs:subClassOf ex:Mammal .
ex:BodyPart a owl:Class ;
  rdfs:label "Body part"@en ;
  rdfs:comment "A part of the body"@en ;
  rdfs:subClassOf ex:AnatomicalStructure .
ex:Function a owl:Class ;
  rdfs:label "Function"@en ;
  rdfs:comment "The natural action or purpose of something"@en ;
  rdfs:subClassOf ex:Characteristic.ex:Mammal a owl:Class ;
  rdfs:label "Mammal"@en ;
  rdfs:comment "A warm-blooded vertebrate animal distinguished by the possession of hair or fur, and females that secrete milk for the nourishment of the young"@en ;
  rdfs:subClassOf ex:Animal .
ex:AnatomicalStructure a owl:Class ;
  rdfs:label "Anatomical structure"@en ;
  rdfs:comment "Any part of an organism, typically a component of macroscopic anatomy"@en .
ex:Characteristic a owl:Class ;
  rdfs:label "Characteristic"@en ;
  rdfs:comment "A feature or quality belonging typically to a person, place, or thing"@en .
ex:Animal a owl:Class ;
  rdfs:label "Animal"@en ;
  rdfs:comment "A multicellular organism that feeds on other organisms in order to survive"@en .
