@prefix xsd: <http://www.w3.org/2001/XMLSchema#> .
@prefix rdf: <http://www.w3.org/1999/02/22-rdf-syntax-ns#> .
@prefix rdfs: <http://www.w3.org/2000/01/rdf-schema#> .
@prefix ex: <http://example.org#> .
ex:Case a rdfs:Class ;
    rdfs:label "Case" ;
    rdfs:comment "A legal or bureaucratic process or event, including all of its related parts and activity"^^xsd:string .
    ex:hasCaseNumber a rdf:Property ;
    rdfs:domain ex:Case ;
    rdfs:range xsd:string ;
    rdfs:label "has case number" ;
    rdfs:comment "The unique identifier given to each case."^^xsd:string .
ex:hasCaseType a rdf:Property ;
    rdfs:domain ex:Case ;
    rdfs:range ex:CaseType ;
    rdfs:label "has case type" ;
    rdfs:comment "The type or classification of a case, defining what kind of process it represents"^^xsd:string .
    ex:CaseType a rdfs:Class ;
    rdfs:label "Case type" ;
    rdfs:comment "The type or classification defining what kind of process a case represents"^^xsd:string .
    ex:hasParty a rdf:Property ;
    rdfs:domain ex:Case ;
    rdfs:range ex:Entity ;
    rdfs:label "has party" ;
    rdfs:comment "An entity involved in a case, for example a person or organization"^^xsd:string .
ex:Entity a rdfs:Class ;
    rdfs:label "Entity" ;
    rdfs:comment "A person or organization involved in a case."^^xsd:string .
    ex:hasStartDate a rdf:Property ;
    rdfs:domain ex:Case ;
    rdfs:range xsd:date ;
    rdfs:label "has start date" ;
    rdfs:comment "The date a case starts."^^xsd:string .
    ex:hasEndDate a rdf:Property ;
    rdfs:domain ex:Case ;
    rdfs:range xsd:date ;
    rdfs:label "has end date" ;
    rdfs:comment "The date a case ends."^^xsd:string .
